Invariant bugs fixed.

Calculus/MultiStaged/Monad.v
@@ -1961,6 +1961,31 @@ Module TranslationProperties (R:Replacement)
     rewrite IHM ; auto.
   Qed.
 
+  Inductive congr_context_ssubst 
+    (P:nat -> CRaw.var -> nat -> T.expr -> nat -> T.expr -> T.expr -> Prop) 
+    (n:nat) (h:CRaw.var)
+    (m:nat) (v:T.expr) (b1 b2:nat) : Context.t -> Context.t -> Prop :=
+  | CongrCSubst_nil : congr_context_ssubst P n h m v b1 b2 nil nil
+  | CongrCSubst_cons : forall (u1 u2:T.expr) (c1 c2:Context.t),
+      P n h m v b1 u1 u2 ->
+      congr_context_ssubst P n h m v b1 b2 c1 c2 ->
+      congr_context_ssubst P n h m v b1 b2
+        (cons (u1,(b2+(length c1))%nat) c1) 
+        (cons (u2,(b2+(length c1))%nat) c2).
+
+  Inductive congr_stack_ssubst 
+    (P:nat -> CRaw.var -> nat -> T.expr -> nat -> T.expr -> T.expr -> Prop) 
+    (n:nat) (h:CRaw.var) (v:T.expr) : 
+    list nat -> nat -> Context.t_stack -> Context.t_stack -> Prop :=
+  | CongrSSubst_nil : forall (bs:list nat) (b:nat), congr_stack_ssubst P n h v bs b nil nil
+  | CongrSSubst_cons_nil: forall (c1 c2:Context.t) (bs:list nat) (b1 b2:nat),
+      congr_context_ssubst P n h 0 v b1 b2 c1 c2 ->
+      congr_stack_ssubst P n h v (b1::bs) b2 (c1::nil) (c2::nil)
+  | CongrSSubst_cons : forall (bs:list nat) (b1 b2:nat) (c1 c2 c1' c2':Context.t) (cs1 cs2:Context.t_stack),
+      congr_context_ssubst P n h (length c1') v b1 b2 c1 c2 ->
+      congr_stack_ssubst P (pred n) h v bs b1 (c1'::cs1) (c2'::cs2) ->
+      congr_stack_ssubst P n h v (b1::bs) b2 (c1::c1'::cs1) (c2::c2'::cs2).
+
   Definition ltb (m n:nat) := leb (S m) n.
 
   Definition admin_ssubst (n:nat) (h:CRaw.var) 
@@ -1974,6 +1999,10 @@ Module TranslationProperties (R:Replacement)
 	  | _ => ss
           end) (M.cast_var (hole_var h)) u1 v) u2.
 
+  Definition admin_context_ssubst := congr_context_ssubst admin_ssubst.
+  Definition admin_stack_ssubst := congr_stack_ssubst admin_ssubst.
+
+(*
   Inductive admin_context_ssubst (n:nat) (h:CRaw.var)
     (m:nat) (v:T.expr) (b1 b2:nat) : Context.t -> Context.t -> Prop :=
   | ACSubst_nil : admin_context_ssubst n h m v b1 b2 nil nil
@@ -1994,6 +2023,7 @@ Module TranslationProperties (R:Replacement)
       admin_context_ssubst n h (length c1') v b1 b2 c1 c2 ->
       admin_stack_ssubst (pred n) h v bs b1 (c1'::cs1) (c2'::cs2) ->
       admin_stack_ssubst n h v (b1::bs) b2 (c1::c1'::cs1) (c2::c2'::cs2).
+*)
 
   Lemma admin_fill_ssubst_1:
     forall (e:S.expr) (bs:list nat),
@@ -2424,27 +2454,23 @@ Module TranslationProperties (R:Replacement)
 	  | _ => ss
           end) (M.cast_var (hole_var h)) u1 v) = u2.
 
-  Inductive eq_context_ssubst (n:nat) (h:CRaw.var)
-    (m:nat) (v:T.expr) (b1 b2:nat) : Context.t -> Context.t -> Prop :=
-  | ECSubst_nil : eq_context_ssubst n h m v b1 b2 nil nil
-  | ECSubst_cons : forall (u1 u2:T.expr) (c1 c2:Context.t),
-      eq_ssubst n h m v b1 u1 u2 ->
-      eq_context_ssubst n h m v b1 b2 c1 c2 ->
-      eq_context_ssubst n h m v b1 b2
-        (cons (u1,(b2+(length c1))%nat) c1) 
-        (cons (u2,(b2+(length c1))%nat) c2).
+  Definition eq_context_ssubst := congr_context_ssubst eq_ssubst.
+  Definition eq_stack_ssubst := congr_stack_ssubst eq_ssubst.
 
-  Inductive eq_stack_ssubst (n:nat) (h:CRaw.var) (v:T.expr) : 
-    list nat -> nat -> Context.t_stack -> Context.t_stack -> Prop :=
-  | ESSubst_nil : forall (bs:list nat) (b:nat), eq_stack_ssubst n h v bs b nil nil
-  | ESSubst_cons_nil: forall (c1 c2:Context.t) (bs:list nat) (b1 b2:nat),
-      eq_context_ssubst n h 0 v b1 b2 c1 c2 ->
-      eq_stack_ssubst n h v (b1::bs) b2 (c1::nil) (c2::nil)
-  | ESSubst_cons : forall (bs:list nat) (b1 b2:nat) (c1 c2 c1' c2':Context.t) (cs1 cs2:Context.t_stack),
-      eq_context_ssubst n h (length c1') v b1 b2 c1 c2 ->
-      eq_stack_ssubst (pred n) h v bs b1 (c1'::cs1) (c2'::cs2) ->
-      eq_stack_ssubst n h v (b1::bs) b2 (c1::c1'::cs1) (c2::c2'::cs2).
+  Definition eq_ssubst_2 (n:nat) (h:CRaw.var) 
+      (m:nat) (v:T.expr) (b:nat) (u1 u2:T.expr) : Prop :=
+      forall (ss:StageSet.t),
+      StageSet.ub n ss = true ->
+      (M.ssubst n (match n with
+	  | S n => if ltb h (b + m) 
+       		then StageSet.add n ss else ss
+	  | _ => ss
+          end) (M.cast_var (hole_var h)) u1 v) = u2.
 
+  Definition eq_context_ssubst_2 := congr_context_ssubst eq_ssubst_2.
+  Definition eq_stack_ssubst_2 := congr_stack_ssubst eq_ssubst_2.
+
+(*
   Definition eq_ssubst_ss (ss:StageSet.t) (n:nat) (h:CRaw.var) 
       (m:nat) (v:T.expr) (b:nat) (u1 u2:T.expr) : Prop :=
       (M.ssubst n (match n with
@@ -2617,7 +2643,7 @@ Module TranslationProperties (R:Replacement)
     assert(ltb h (b + m) = false).
     apply leb_iff_conv ; apply leb_iff_conv in Heqb0 ; omega.
     rewrite H1 in H ; auto.
-  Qed.
+  Qed.*)
 
   Lemma eq_ssubst_m_Sm:
     forall (e:T.expr) (b:nat) (h:S.var) (v:T.expr) (n m:nat),
@@ -2645,6 +2671,33 @@ Module TranslationProperties (R:Replacement)
     rewrite Eq1 ; apply H ; auto.
   Qed.
 
+  Lemma eq_ssubst_2_m_Sm:
+    forall (e:T.expr) (b:nat) (h:S.var) (v:T.expr) (n m:nat),
+    eq_ssubst_2 n h m v b e e -> eq_ssubst_2 n h (S m) v b e e.
+  Proof.
+    unfold eq_ssubst_2 ; intros.
+    case_beq_nat h (b + m)%nat.
+    assert(ltb (b+m)%nat (b + m)%nat = false) as LtbFalse.
+    apply leb_iff_conv ; omega.
+    rewrite LtbFalse in H.
+    assert(ltb (b+m)%nat (b + S m)%nat = true) as LtbTrue.
+    apply leb_iff ; omega.
+    rewrite LtbTrue.
+    destruct n.
+    apply H ; auto.
+    apply H ; auto.
+    rewrite <- StageSetProperties.ub_le_1 ; auto.
+    destruct n.
+    apply H ; auto.
+    assert(ltb h (b + S m) = ltb h (b + m)) as Eq1.
+    generalize E ; clear ; intros.
+    remember (ltb h (b + m)) ; destruct b0 ; symmetry in Heqb0 ;
+    [apply leb_iff ; apply leb_iff in Heqb0 | 
+    apply leb_iff_conv ; apply leb_iff_conv in Heqb0] ; omega.
+    rewrite Eq1 ; apply H ; auto.
+  Qed.
+
+(*
   Lemma eq_context_ssubst_ss_m_ge:
     forall (c:Context.t) (b1 b2:nat) (h:S.var) (v:T.expr) (n m p:nat) (ss:StageSet.t),
     eq_context_ssubst_ss (match n with
@@ -2662,6 +2715,8 @@ Module TranslationProperties (R:Replacement)
     apply IHc with (m:=m) ; auto.
   Qed.
 
+  *)
+
   Lemma eq_ssubst_m_ge:
     forall (e:T.expr) (b:nat) (h:S.var) (v:T.expr) (n m p:nat),
     eq_ssubst n h m v b e e -> 
@@ -2672,20 +2727,42 @@ Module TranslationProperties (R:Replacement)
     apply eq_ssubst_m_Sm ; auto.
   Qed.
 
+  Lemma eq_ssubst_2_m_ge:
+    forall (e:T.expr) (b:nat) (h:S.var) (v:T.expr) (n m p:nat),
+    eq_ssubst_2 n h m v b e e -> 
+    m <= p -> eq_ssubst_2 n h p v b e e.
+  Proof.
+    intros.
+    induction H0 ; auto.
+    apply eq_ssubst_2_m_Sm ; auto.
+  Qed.
+
   Lemma eq_context_ssubst_m_ge:
     forall (c:Context.t) (b1 b2:nat) (h:S.var) (v:T.expr) (n m p:nat),
     eq_context_ssubst n h m v b1 b2 c c -> 
     m <= p -> eq_context_ssubst n h p v b1 b2 c c.
   Proof.
     intros.
-    induction H0 ; auto.
     induction c ; auto.
     constructor.
     inversion H ; subst.
     constructor ; auto.
     apply eq_ssubst_m_ge with (m:=m) ; auto.
-    inversion IHle ; subst.
-    auto.
+    apply IHc ; auto.
+  Qed.
+
+  Lemma eq_context_ssubst_2_m_ge:
+    forall (c:Context.t) (b1 b2:nat) (h:S.var) (v:T.expr) (n m p:nat),
+    eq_context_ssubst_2 n h m v b1 b2 c c -> 
+    m <= p -> eq_context_ssubst_2 n h p v b1 b2 c c.
+  Proof.
+    intros.
+    induction c ; auto.
+    constructor.
+    inversion H ; subst.
+    constructor ; auto.
+    apply eq_ssubst_2_m_ge with (m:=m) ; auto.
+    apply IHc ; auto.
   Qed.
 
   Lemma eq_ssubst_fill_gt_1_strong:
@@ -3007,24 +3084,314 @@ Module TranslationProperties (R:Replacement)
     rewrite StageSetProperties.ub_le_2 with (m:=S (S m)) ; auto.
   Qed.
 
-  Lemma eq_ssubst_context_app:
-    forall (c1 c2:Context.t) (n m b1 b2:nat) (h:S.var) (v:T.expr),
-    eq_context_ssubst n h m v b1 (b2 + length c2) c1 c1 ->
-    eq_context_ssubst n h m v b1 b2 c2 c2 ->
-    eq_context_ssubst n h m v b1 b2 (c1 ++ c2) (c1 ++ c2).
+  Lemma eq_ssubst_2_fill_ge_1_strong:
+    forall (e:S.expr) (bs:list nat) (h:S.var) (v:T.expr),
+    let (e0, cs) := trans e (0::bs) in
+    match cs with
+    | c1 :: nil => 
+      match c1 with
+      | nil => False
+      | _ => forall (m:nat), 
+        0 <= m < length bs ->
+        let b := hd 0 bs in
+        eq_context_ssubst_2 m h 0 v b 0 c1 c1 ->
+        forall (ss:StageSet.t),
+        StageSet.ub m ss = true ->
+        (M.ssubst (S m) (match (S m) with
+	  | S m => if ltb h (length c1)
+       		then StageSet.add m 
+                (match m with
+                | 0 => ss
+                | S m0 =>
+                    if ltb h (b + 0) then StageSet.add m0 ss else ss
+                end)
+                else 
+                (match m with
+                | 0 => ss
+                | S m0 =>
+                    if ltb h (b + 0) then StageSet.add m0 ss else ss
+                end)
+	  | _ => (match m with
+                | 0 => ss
+                | S m0 =>
+                    if ltb h (b + 0) then StageSet.add m0 ss else ss
+                end)
+          end)  (M.cast_var (hole_var h)) e0 v) = e0 ->
+        (M.ssubst m (match m with
+	  | S m => if ltb h (b + 0) 
+       		then StageSet.add m ss else ss
+	  | _ => ss
+          end) (M.cast_var (hole_var h)) (Context.fill c1 (ret (cast_ebox e0))) v) = 
+          (Context.fill c1 (ret (cast_ebox e0)))
+      end
+    | _ => True
+    end.
   Proof.
-    induction c1 ; simpl ; intros ; auto.
-    inversion H ; subst.
-    assert((b2 + length c2 + length c1) = b2 + (length (c1++c2)))%nat as Eq1.
-    rewrite app_length ; simpl ; omega.
-    rewrite Eq1 ; constructor ; auto.
+    intros.
+    specialize (context_stack_not_nil e (0::bs)) ; intros CSNotNil.
+    destruct (trans e (0::bs)).
+    destruct t ; auto.
+    destruct t0 ; auto.
+    destruct t ; auto.
+    exfalso ; apply CSNotNil ; simpl ; auto.
+    simpl ; intros.
+
+    simpl in *|-*.
+    inversion H0.
+    subst c1 u2 c2 p.
+    clear H0 CSNotNil.
+    destruct bs ; [exfalso ; generalize H ; clear ; simpl ; intros ; omega|].
+    simpl in *|-*.
+    generalize dependent u1 ; generalize dependent ss.
+    induction t ; simpl ; unfold eq_ssubst_2 ; intros.
+
+    rewrite MP.ssubst_bind with (f2:=
+    (fun v0 : T.expr =>
+      cast_eapp (cast_eabs (cast_var (hole_var 0)) (ret (cast_ebox e0))) v0)).
+    rewrite H6 ; auto.
+    intros.
+    rewrite MP.ssubst_eapp, MP.ssubst_eabs, MP.ssubst_ret, MP.ssubst_ebox.
+    simpl in *|-*.
+
+    assert(beq_var (hole_var h) (hole_var 0) = ltb h 1) as Eq1.
+    clear ; simpl ; remember (ltb h 1) ; destruct b ; symmetry in Heqb.
+    apply beq_nat_true_iff ; apply leb_iff in Heqb ; unfold hole_var ; omega.
+    apply beq_nat_false_iff ; apply leb_iff_conv in Heqb ; unfold hole_var ; omega.
+    destruct m ; destruct (ltb h (n + 0)) ; rewrite Eq1, H2 ; auto.
+
+    inversion H8 ; clear H8.
+    subst c1 u2 c2 a.
+
+    rewrite MP.ssubst_bind with (f2:=(fun v0 : T.expr =>
+     cast_eapp
+     (cast_eabs (cast_var (hole_var (S (length t))))
+        (bind u0
+           (fun v1 : T.expr =>
+            cast_eapp
+              (cast_eabs (cast_var (hole_var (length t)))
+                 (Context.fill t (ret (cast_ebox e0)))) v1))) v0)).
+    rewrite H6 ; auto.
+    intros.
+    rewrite MP.ssubst_eapp, MP.ssubst_eabs.
+    simpl in *|-*.
+
+      (* Case h = S length t *)
+      case_beq_nat h (S (length t)).
+      rewrite <- beq_nat_refl.
+      assert(ltb (S (length t)) (S (length t)) = false) as False1.
+      apply leb_iff_conv ; omega.
+      rewrite False1 in IHt.
+      assert(ltb (S (length t)) (S (S (length t))) = true) as True1.
+      apply leb_iff ; omega.
+      rewrite True1 in H2.
+      destruct m ; [| destruct (ltb (S (length t)) (n + 0)) ] ;
+      try(rewrite StageSetProperties.add_add) ; rewrite IHt ; auto ;
+      try(rewrite StageSetProperties.add_mem_4 ; auto) ;
+      try(rewrite <- StageSetProperties.ub_le_1 ; auto).
+      rewrite StageSetProperties.add_add ; auto.
+
+      (* Case h < S length t *)
+      assert(beq_var (hole_var h) (hole_var (S (length t))) = false) as False1.
+      apply beq_nat_false_iff ; unfold hole_var ; omega.
+      rewrite False1, IHt ; auto.
+      assert(ltb h (S (length t)) = ltb h (S (S (length t)))) as Eq1.
+      remember (ltb h (S (S (length t)))) ; destruct b ; symmetry in Heqb.
+      apply leb_iff ; apply leb_iff in Heqb ; omega.
+      apply leb_iff_conv ; apply leb_iff_conv in Heqb ; omega.
+      rewrite Eq1 ; auto.
   Qed.
 
-  Lemma eq_ssubst_context_ss_app:
-    forall (c1 c2:Context.t) (n m b1 b2:nat) (h:S.var) (v:T.expr) (ss:StageSet.t),
-    eq_context_ssubst_ss ss n h m v b1 (b2 + length c2) c1 c1 ->
-    eq_context_ssubst_ss ss n h m v b1 b2 c2 c2 ->
-    eq_context_ssubst_ss ss n h m v b1 b2 (c1 ++ c2) (c1 ++ c2).
+  Lemma eq_ssubst_2_fill_ge_1:
+    forall (e:S.expr) (bs:list nat) (h:S.var) (v:T.expr),
+    let (e0, cs) := trans e (0::bs) in
+    match cs with
+    | c1 :: nil => 
+      match c1 with
+      | nil => False
+      | _ => forall (m:nat), 
+        0 <= m < length bs ->
+        let b := hd 0 bs in
+        eq_ssubst_2 (S m) h (length c1) v 0 e0 e0 ->
+        eq_context_ssubst_2 m h 0 v b 0 c1 c1 ->
+        eq_ssubst_2 m h 0 v b
+        (Context.fill c1 (ret (cast_ebox e0))) (Context.fill c1 (ret (cast_ebox e0)))
+      end
+    | _ => True
+    end.
+  Proof.
+    intros.
+    specialize (eq_ssubst_2_fill_ge_1_strong e bs) ; intros Strong1.
+    specialize (context_stack_not_nil e (0::bs)) ; intros CSNotNil.
+    destruct (trans e (0::bs)).
+    destruct t ; auto.
+    destruct t0 ; auto.
+    destruct t ; auto.
+    unfold eq_ssubst_2 ; intros.
+    apply Strong1 ; auto.
+    simpl plus in *|-* ; simpl length in *|-*.
+    destruct m.
+    apply H0 ; auto.
+    rewrite StageSetProperties.ub_le_2 with (m:=0) ; auto.
+    apply H0 ; auto.
+    destruct (ltb h (hd 0 bs + 0)) ; [
+    rewrite <- StageSetProperties.ub_le_1 ; auto |] ;
+    rewrite StageSetProperties.ub_le_2 with (m:=S m) ; auto.
+  Qed.
+
+
+  Lemma eq_ssubst_2_fill_ge_2_strong:
+    forall (e:S.expr) (bs:list nat) (h:S.var) (v:T.expr),
+    let (e0, cs) := trans e (0::bs) in
+    match cs with
+    | c1 :: c1' :: cs => 
+      match c1 with
+      | nil => False
+      | _ => forall (m:nat), 
+        S (length cs) <= m < length bs ->
+        let b := hd 0 bs in
+        eq_context_ssubst_2 m h (length c1') v b 0 c1 c1 ->
+        forall (ss:StageSet.t),
+        StageSet.ub m ss = true ->
+        (M.ssubst (S m) (match (S m) with
+	  | S (S m) => if ltb h (0 + (length c1)) 
+       		then StageSet.add (S m) (if ltb h (b + length c1')
+                      then StageSet.add m ss
+                      else ss) 
+                else (if ltb h (b + length c1') then StageSet.add m ss
+                      else ss)
+	  | _ => ss
+          end) (M.cast_var (hole_var h)) e0 v) = e0 ->
+
+        (M.ssubst m (match m with
+	  | S m => if ltb h (b + (length c1')) 
+       		then StageSet.add m ss else ss
+	  | _ => ss
+          end) (M.cast_var (hole_var h)) (Context.fill c1 (ret (cast_ebox e0))) v) = 
+          (Context.fill c1 (ret (cast_ebox e0)))
+      end
+    | _ => True
+    end.
+  Proof.
+    intros.
+    specialize (context_stack_not_nil e (0::bs)) ; intros CSNotNil.
+    destruct (trans e (0::bs)).
+    destruct t ; auto.
+    destruct t0 ; auto.
+    destruct t ; auto.
+    exfalso ; apply CSNotNil ; simpl ; auto.
+    simpl ; intros.
+
+    simpl in *|-*.
+    
+    inversion H0.
+    subst c1 u2 c2 p.
+    clear H0 CSNotNil.
+    destruct bs ; [exfalso ; generalize H ; clear ; simpl ; intros ; omega|].
+    simpl in *|-*.
+    generalize dependent u1 ; generalize dependent ss.
+    induction t ; simpl ; unfold eq_ssubst ; intros.
+
+    destruct m ; [exfalso ; omega|].
+    rewrite MP.ssubst_bind with (f2:=
+    (fun v0 : T.expr =>
+      cast_eapp (cast_eabs (cast_var (hole_var 0)) (ret (cast_ebox e0))) v0)).
+    rewrite H6 ; auto.
+    intros.
+    rewrite MP.ssubst_eapp, MP.ssubst_eabs, MP.ssubst_ret, MP.ssubst_ebox.
+    simpl in *|-*.
+
+    assert(beq_var (hole_var h) (hole_var 0) = ltb h 1) as Eq1.
+    clear ; simpl ; remember (ltb h 1) ; destruct b ; symmetry in Heqb.
+    apply beq_nat_true_iff ; apply leb_iff in Heqb ; unfold hole_var ; omega.
+    apply beq_nat_false_iff ; apply leb_iff_conv in Heqb ; unfold hole_var ; omega.
+    destruct m ; destruct (ltb h (n + (length t0))) ; rewrite Eq1, H2 ; auto.
+
+    inversion H8 ; clear H8.
+    subst c1 u2 c2 a.
+    destruct m ; [exfalso ; omega|].
+
+    rewrite MP.ssubst_bind with (f2:=(fun v0 : T.expr =>
+     cast_eapp
+     (cast_eabs (cast_var (hole_var (S (length t))))
+        (bind u0
+           (fun v1 : T.expr =>
+            cast_eapp
+              (cast_eabs (cast_var (hole_var (length t)))
+                 (Context.fill t (ret (cast_ebox e0)))) v1))) v0)).
+    rewrite H6 ; auto.
+    intros.
+    rewrite MP.ssubst_eapp, MP.ssubst_eabs.
+    simpl in *|-*.
+
+      (* Case h = S length t *)
+      case_beq_nat h (S (length t)).
+      rewrite <- beq_nat_refl.
+      assert(ltb (S (length t)) (S (length t)) = false) as False1.
+      apply leb_iff_conv ; omega.
+      rewrite False1 in IHt.
+      assert(ltb (S (length t)) (S (S (length t))) = true) as True1.
+      apply leb_iff ; omega.
+      rewrite True1 in H2.
+      destruct (ltb (S (length t)) (n + (length t0))) ;
+      try(rewrite StageSetProperties.add_add) ; rewrite IHt ; auto ;
+      try(rewrite StageSetProperties.add_mem_4 ; auto) ;
+      try(rewrite <- StageSetProperties.ub_le_1 ; auto).
+      rewrite StageSetProperties.add_add ; auto.
+
+      (* Case h < S length t *)
+      assert(beq_var (hole_var h) (hole_var (S (length t))) = false) as False1.
+      apply beq_nat_false_iff ; unfold hole_var ; omega.
+      rewrite False1, IHt ; auto.
+      assert(ltb h (S (length t)) = ltb h (S (S (length t)))) as Eq1.
+      remember (ltb h (S (S (length t)))) ; destruct b ; symmetry in Heqb.
+      apply leb_iff ; apply leb_iff in Heqb ; omega.
+      apply leb_iff_conv ; apply leb_iff_conv in Heqb ; omega.
+      rewrite Eq1 ; auto.
+  Qed.
+
+  Lemma eq_ssubst_2_fill_ge_2:
+    forall (e:S.expr) (bs:list nat) (h:S.var) (v:T.expr),
+    let (e0, cs) := trans e (0::bs) in
+    match cs with
+    | c1 :: c1' :: cs => 
+      match c1 with
+      | nil => False
+      | _ => forall (m:nat), 
+        S (length cs) <= m < length bs ->
+        let b := hd 0 bs in
+        eq_ssubst_2 (S m) h (length c1) v 0 e0 e0 ->
+        eq_context_ssubst_2 m h (length c1') v b 0 c1 c1 ->
+        eq_ssubst_2 m h (length c1') v b
+        (Context.fill c1 (ret (cast_ebox e0))) (Context.fill c1 (ret (cast_ebox e0)))
+      end
+    | _ => True
+    end.
+  Proof.
+    intros.
+    specialize (eq_ssubst_2_fill_ge_2_strong e bs) ; intros Strong1.
+    specialize (context_stack_not_nil e (0::bs)) ; intros CSNotNil.
+    destruct (trans e (0::bs)).
+    destruct t ; auto.
+    destruct t0 ; auto.
+    destruct t ; auto.
+    unfold eq_ssubst_2 ; intros.
+    apply Strong1 ; auto.
+    simpl plus in *|-* ; simpl length in *|-*.
+    clear Strong1 CSNotNil.
+    destruct m ; [exfalso ; omega|].
+    apply H0 ; auto.
+
+    destruct (ltb h (hd 0 bs + (length t0))) ; [
+    rewrite <- StageSetProperties.ub_le_1 ; auto |] ;
+    rewrite StageSetProperties.ub_le_2 with (m:=S m) ; auto.
+  Qed.
+
+  Lemma congr_ssubst_context_app:
+    forall (P:nat -> CRaw.var -> nat -> T.expr -> nat -> T.expr -> T.expr -> Prop)
+    (c1 c2:Context.t) (n m b1 b2:nat) (h:S.var) (v:T.expr),
+    congr_context_ssubst P n h m v b1 (b2 + length c2) c1 c1 ->
+    congr_context_ssubst P n h m v b1 b2 c2 c2 ->
+    congr_context_ssubst P n h m v b1 b2 (c1 ++ c2) (c1 ++ c2).
   Proof.
     induction c1 ; simpl ; intros ; auto.
     inversion H ; subst.
@@ -3044,13 +3411,13 @@ Module TranslationProperties (R:Replacement)
     apply H ; auto.
   Qed.
 
-  Lemma eq_ssubst_ss_sum:
-    forall (e v:T.expr) (n m1 m2 b1 b2:nat) (h:S.var) (ss:StageSet.t),
-    eq_ssubst_ss ss n h m1 v b1 e e ->
+  Lemma eq_ssubst_2_sum:
+    forall (e v:T.expr) (n m1 m2 b1 b2:nat) (h:S.var),
+    eq_ssubst_2 n h m1 v b1 e e ->
     (b1 + m1 = b2 + m2)%nat ->
-    eq_ssubst_ss ss n h m2 v b2 e e.
+    eq_ssubst_2 n h m2 v b2 e e.
   Proof.
-    unfold eq_ssubst_ss ; intros.
+    unfold eq_ssubst_2 ; intros.
     rewrite <- H0.
     apply H ; auto.
   Qed.
@@ -3068,18 +3435,18 @@ Module TranslationProperties (R:Replacement)
     apply eq_ssubst_sum with (m1:=m1) (b1:=b1) ; auto.
     apply IHc with (m1:=m1) (b1:=b1) ; auto.
   Qed.
-  
-  Lemma eq_context_ssubst_ss_sum:
-    forall (c:Context.t) (v:T.expr) (n m1 m2 b1 b2 b3:nat) (h:S.var) (ss:StageSet.t),
-    eq_context_ssubst_ss ss n h m1 v b1 b3 c c ->
+
+  Lemma eq_context_ssubst_2_sum:
+    forall (c:Context.t) (v:T.expr) (n m1 m2 b1 b2 b3:nat) (h:S.var),
+    eq_context_ssubst_2 n h m1 v b1 b3 c c ->
     (b1 + m1 = b2 + m2)%nat ->
-    eq_context_ssubst_ss ss n h m2 v b2 b3 c c.
+    eq_context_ssubst_2 n h m2 v b2 b3 c c.
   Proof.
     induction c ; simpl ; intros.
     constructor.
     inversion H ; subst.
     constructor ; auto.
-    apply eq_ssubst_ss_sum with (m1:=m1) (b1:=b1) ; auto.
+    apply eq_ssubst_2_sum with (m1:=m1) (b1:=b1) ; auto.
     apply IHc with (m1:=m1) (b1:=b1) ; auto.
   Qed.
 
@@ -3153,27 +3520,121 @@ Module TranslationProperties (R:Replacement)
     inversion H0 ; subst ; [simpl in *|-*|].
     inversion H1 ; subst ; simpl in *|-*.
     constructor ; auto.
-    apply eq_ssubst_context_app ; auto.
+    apply congr_ssubst_context_app ; auto.
     rewrite plus_0_r in H5 ; auto.
 
     constructor ; auto.
-    apply eq_ssubst_context_app ; auto.
+    apply congr_ssubst_context_app ; auto.
     apply eq_context_ssubst_sum with (m1:=0) (b1:=(n0 + length c1')%nat) ; auto.
 
     inversion H1 ; subst.
     simpl ; constructor ; auto.
-    apply eq_ssubst_context_app ; simpl in *|-* ; auto.
+    apply congr_ssubst_context_app ; simpl in *|-* ; auto.
     simpl in *|-* ; rewrite plus_0_r in H6 ; auto.
     apply eq_context_ssubst_m_ge with (m:=0) ; auto ; omega.
 
     constructor ; auto.
-    apply eq_ssubst_context_app ; auto.
+    apply congr_ssubst_context_app ; auto.
 
     simpl in *|-* ; auto.
     apply eq_context_ssubst_sum with (m1:=length c1') (b1:=(n0 + length c1'0)%nat) ; auto.
     rewrite app_length ; omega.
 
     apply eq_context_ssubst_m_ge with (m:=length c1'0) ; auto.
+    rewrite app_length ; omega.
+  Qed.
+
+  Lemma eq_ssubst_2_merge:
+    forall (e1 e2:S.expr) (bs:list nat) (h:S.var) (v:T.expr),
+    let (e1', cs1) := trans e1 (map_iter_booker e2 bs 0) in
+    let (e2', cs2) := trans e2 bs in
+    forall (m:nat),
+    max (depth e1) (depth e2) <= m < length bs ->
+    eq_stack_ssubst_2 (pred m) h v (tl (map_iter_booker e2 bs 0))
+       (hd 0 (map_iter_booker e2 bs 0)) cs1 cs1 ->
+    eq_stack_ssubst_2 (pred m) h v (tl bs) (hd 0 bs) cs2 cs2 ->
+    eq_stack_ssubst_2 (pred m) h v (tl bs) (hd 0 bs) (Context.merge cs1 cs2)
+      (Context.merge cs1 cs2).
+  Proof.
+    intros.
+    specialize (map_iter_booker_stack e2 bs) ; intros MapIterBooker2.
+    specialize (depth_length e1 (map_iter_booker e2 bs 0)) ; intros DpthLength1.
+    specialize (depth_length e2 bs) ; intros DpthLength2.
+    destruct (trans e1) ; destruct (trans e2) ; intros.
+    rewrite DpthLength1, DpthLength2 in H ; clear DpthLength1 DpthLength2.
+    rewrite MapIterBooker2 in H0 ; clear MapIterBooker2.
+    
+    generalize dependent m ; generalize dependent t ;
+    generalize dependent bs.
+    induction t0 ; simpl ; intros ; auto.
+    rewrite ContextStaticProperties.merge_nil_r ; simpl ; auto.
+    destruct bs ; [exfalso ; simpl in *|-* ; omega|].
+
+    assert(forall (bs:list nat) (m:nat), bs = 
+      (tl (map_iter_stack nil (n :: bs) m))) as Eq1.
+    induction bs0 ; simpl in *|-* ; intros ; auto.
+    rewrite <- IHbs0 ; auto.
+    rewrite plus_0_r ; simpl ; auto.
+
+    rewrite <- Eq1 in H0.
+    simpl in *|-* ; rewrite plus_0_r in H0 ; auto.
+
+    destruct bs ; [exfalso ; simpl in *|-* ; omega|].
+    destruct t ; [simpl in *|-* |] ; auto.
+    destruct m ; [simpl in *|-* ; exfalso ; omega|].
+    destruct bs ; [exfalso ; simpl in *|-* ; omega|].
+
+    specialize (IHt0 (n0::bs) t1).
+    simpl in IHt0.
+    assert(eq_stack_ssubst_2 (pred m) h v bs n0 (Context.merge t1 t0)
+         (Context.merge t1 t0)) as IH.
+    apply IHt0 ; auto.
+    simpl in H ; omega.
+
+    
+    assert(forall (bs:list nat) (n0 m:nat), 
+      map_iter_stack t0 (n0 :: bs) m = 
+      tl (map_iter_stack (a :: t0) (n :: n0 :: bs) m)) as Eq2.
+    induction bs0 ; simpl in *|-* ; intros ; auto.
+    unfold map_iter_stack in *|-* ; simpl.
+    specialize (IHbs0 a0 (S m0)).
+    simpl in IHbs0.
+    rewrite IHbs0 ; auto.
+    rewrite <- Eq2 in H0.
+    inversion H0 ; subst ; auto.
+    constructor.
+
+    simpl in *|-*.
+    inversion H1 ; subst ; auto.
+    constructor.
+    clear IHt0.
+
+    simpl in *|-*.
+
+    inversion H0 ; subst ; [simpl in *|-*|].
+    inversion H1 ; subst ; simpl in *|-*.
+    constructor ; auto.
+    apply congr_ssubst_context_app ; auto.
+    rewrite plus_0_r in H5 ; auto.
+
+    constructor ; auto.
+    apply congr_ssubst_context_app ; auto.
+    apply eq_context_ssubst_2_sum with (m1:=0) (b1:=(n0 + length c1')%nat) ; auto.
+
+    inversion H1 ; subst.
+    simpl ; constructor ; auto.
+    apply congr_ssubst_context_app ; simpl in *|-* ; auto.
+    simpl in *|-* ; rewrite plus_0_r in H6 ; auto.
+    apply eq_context_ssubst_2_m_ge with (m:=0) ; auto ; omega.
+
+    constructor ; auto.
+    apply congr_ssubst_context_app ; auto.
+
+    simpl in *|-* ; auto.
+    apply eq_context_ssubst_2_sum with (m1:=length c1') (b1:=(n0 + length c1'0)%nat) ; auto.
+    rewrite app_length ; omega.
+
+    apply eq_context_ssubst_2_m_ge with (m:=length c1'0) ; auto.
     rewrite app_length ; omega.
   Qed.
 
@@ -3545,288 +4006,16 @@ Module TranslationProperties (R:Replacement)
     inversion H0.
   Qed.
 
-  Lemma eq_ssubst_fill_eq_1:
-    forall (e:S.expr) (bs:list nat) (h:S.var) (v:T.expr),
-    let (e0, cs) := trans e (0::bs) in
-    match cs with
-    | c1 :: nil => 
-      match c1 with
-      | nil => False
-      | _ => forall (ss:StageSet.t), 
-        0 < length bs ->
-        h < length c1 ->
-        let b := hd 0 bs in
-        eq_ssubst_ss (StageSet.add 0 ss) 1 h (length c1) v 0 e0 e0 ->
-        eq_context_ssubst_ss (StageSet.remove 1 (StageSet.add 0 ss)) 0 h 0 v b 0 c1 c1 ->
-        eq_ssubst_ss ss 0 h 0 v b
-        (Context.fill c1 (ret (cast_ebox e0))) (Context.fill c1 (ret (cast_ebox e0)))
-      end
-    | _ => True
-    end.
-  Proof.
-    admit. (* todo *)
-  Qed.
-
-  Lemma eq_ssubst_fill_eq_2:
-    forall (e:S.expr) (bs:list nat) (h:S.var) (v:T.expr),
-    let (e0, cs) := trans e (0::bs) in
-    match cs with
-    | c1 :: nil => 
-      match c1 with
-      | nil => False
-      | _ => forall (ss:StageSet.t), 
-        0 < length bs ->
-        length c1 <= h ->
-        let b := hd 0 bs in
-        eq_ssubst_ss ss 1 h (length c1) v 0 e0 e0 ->
-        eq_context_ssubst_ss (StageSet.remove 1 ss) 0 h 0 v b 0 c1 c1 ->
-        eq_ssubst_ss ss 0 h 0 v b
-        (Context.fill c1 (ret (cast_ebox e0))) (Context.fill c1 (ret (cast_ebox e0)))
-      end
-    | _ => True
-    end.
-  Proof.
-    admit. (* todo *)
-  Qed.
-
-  Lemma eq_ssubst_fill_eq_3:
-    forall (e:S.expr) (bs:list nat) (h:S.var) (v:T.expr),
-    let (e0, cs) := trans e (0::bs) in
-    match cs with
-    | c1 :: c2 :: cs => 
-      match c1 with
-      | nil => False
-      | _ => forall (ss:StageSet.t), 
-        S (length cs) < length bs ->
-        let b := hd 0 bs in
-        eq_ssubst_ss ss (S (S (length cs))) h (length c1) v 0 e0 e0 ->
-        eq_context_ssubst_ss (StageSet.remove (S (S (length cs))) ss) (S (length cs)) h (length c2) v b 0 c1 c1 ->
-        eq_ssubst_ss ss (S (length cs)) h (length c2) v b
-        (Context.fill c1 (ret (cast_ebox e0))) (Context.fill c1 (ret (cast_ebox e0)))
-      end
-    | _ => True
-    end.
-  Proof.
-    admit. (* todo *)
-  Qed.
-
-  Lemma eq_ssubst_ss_merge:
-    forall (e1 e2:S.expr) (bs:list nat) (h:S.var) (v:T.expr),
-    let (e1', cs1) := trans e1 (map_iter_booker e2 bs 0) in
-    let (e2', cs2) := trans e2 bs in
-    forall (m:nat),
-    max (depth e1) (depth e2) <= m < length bs ->
-    (forall (ss:StageSet.t),
-    StageSet.ub (pred m) ss = true ->
-    StageSet.mem 0 ss = true ->
-    eq_stack_ssubst_ss ss (pred m) h v (tl (map_iter_booker e2 bs 0))
-       (hd 0 (map_iter_booker e2 bs 0)) cs1 cs1) ->
-    (forall (ss:StageSet.t),
-    StageSet.ub (pred m) ss = true ->
-    StageSet.mem 0 ss = true ->
-    eq_stack_ssubst_ss ss (pred m) h v (tl bs) (hd 0 bs) cs2 cs2) ->
-    (forall (ss:StageSet.t),
-    StageSet.ub (pred m) ss = true ->
-    StageSet.mem 0 ss = true ->
-    eq_stack_ssubst_ss ss (pred m) h v (tl bs) (hd 0 bs) (Context.merge cs1 cs2)
-      (Context.merge cs1 cs2)).
-  Proof.
-    intros.
-    specialize (map_iter_booker_stack e2 bs) ; intros MapIterBooker2.
-    specialize (depth_length e1 (map_iter_booker e2 bs 0)) ; intros DpthLength1.
-    specialize (depth_length e2 bs) ; intros DpthLength2.
-    destruct (trans e1) ; destruct (trans e2) ; intros.
-    rewrite DpthLength1, DpthLength2 in H ; clear DpthLength1 DpthLength2.
-    rewrite MapIterBooker2 in H0 ; clear MapIterBooker2.
-    
-    generalize dependent ss ; generalize dependent m ; generalize dependent t ;
-    generalize dependent bs.
-    induction t0 ; simpl ; intros ; auto.
-    rewrite ContextStaticProperties.merge_nil_r ; simpl ; auto.
-    destruct bs ; [exfalso ; simpl in *|-* ; omega|].
-
-    assert(forall (bs:list nat) (m:nat), bs = 
-      (tl (map_iter_stack nil (n :: bs) m))) as Eq1.
-    induction bs0 ; simpl in *|-* ; intros ; auto.
-    rewrite <- IHbs0 ; auto.
-    rewrite plus_0_r ; simpl ; auto.
-
-    rewrite <- Eq1 in H0.
-    simpl in *|-* ; rewrite plus_0_r in H0 ; auto.
-
-    destruct bs ; [exfalso ; simpl in *|-* ; omega|].
-    destruct t ; [simpl in *|-* |] ; auto.
-    destruct m ; [simpl in *|-* ; exfalso ; omega|].
-    destruct bs ; [exfalso ; simpl in *|-* ; omega|].
-
-    simpl.
-
-    specialize (IHt0 (n0::bs) t1).
-    simpl in IHt0.
-
-    destruct m ; auto.
-
-    (* Case m = 0 *)
-    simpl in H.
-    destruct t1 ; destruct t0 ; simpl in *|-* ; try(exfalso ; omega).
-    constructor ; auto.
-    apply eq_ssubst_context_ss_app ; auto.
-    specialize (H0 ss H2 H3).
-    inversion H0 ; subst ; auto.
-    rewrite plus_0_r in H7 ; auto.
-    specialize (H1 ss H2 H3).
-    inversion H1 ; subst ; auto.
-
-    (* Case m > 0 *)
-    assert(eq_stack_ssubst_ss (StageSet.remove (S m) ss) (pred (S m)) h v bs n0 (Context.merge t1 t0)
-         (Context.merge t1 t0)) as IH.
-    apply IHt0 ; auto ; intros.
-    intros.
-    simpl in H ; omega.
-    destruct t1 ; [constructor|] ; auto.
-    assert(StageSet.ub (S m) ss0 = true) as Ub1.
-    rewrite StageSetProperties.ub_le_2 with (m:=m) ; auto ; omega.
-    specialize (H0 ss0 Ub1 H5).
-
-    assert(forall (bs:list nat) (n0 m:nat), 
-      map_iter_stack t0 (n0 :: bs) m = 
-      tl (map_iter_stack (a :: t0) (n :: n0 :: bs) m)) as Eq2.
-    induction bs0 ; simpl in *|-* ; intros ; auto.
-    unfold map_iter_stack in *|-* ; simpl.
-    specialize (IHbs0 a0 (S m0)).
-    simpl in IHbs0.
-    rewrite IHbs0 ; auto.
-    rewrite <- Eq2 in H0.
-    inversion H0 ; subst ; auto.
-    rewrite StageSetProperties.remove_equal in H16 ; auto.
-    rewrite StageSetProperties.ub_mem_1 with (m:=m) ; auto.
-
-    destruct t0 ; [constructor|].
-    assert(StageSet.ub (S m) ss0 = true) as Ub1.
-    rewrite StageSetProperties.ub_le_2 with (m:=m) ; auto ; omega.
-    specialize (H1 ss0 Ub1 H5).
-
-    inversion H1 ; subst ; auto.
-    rewrite StageSetProperties.remove_equal in H16 ; auto.
-    rewrite StageSetProperties.ub_mem_1 with (m:=m) ; auto.
-
-    rewrite <- StageSetProperties.ub_pred ; auto.
-    rewrite StageSetProperties.remove_mem_1 ; auto.
-
-    simpl in *|-*.
-
-    destruct t0 ; subst ; [simpl in *|-*|].
-    destruct t1 ; subst ; simpl in *|-*.
-    constructor ; auto.
-    apply eq_ssubst_context_ss_app ; auto.
-    specialize (H0 ss H2 H3).
-    inversion H0 ; subst ; rewrite plus_0_r in *|-* ; auto.
-    specialize (H1 ss H2 H3).
-    inversion H1 ; subst ; auto.
-
-    constructor ; auto.
-    apply eq_ssubst_context_ss_app ; auto.
-    specialize (H0 ss H2 H3).
-    inversion H0 ; subst.
-    rewrite plus_0_r in *|-* ; auto.
-
-    specialize (H1 match (S m) with
-    | 0 => ss
-    | 1 => ss
-    | S (S n2) => if ltb h (n0 + length t0) then StageSet.add (S n2) ss else ss
-    end).
-    assert(StageSet.ub (S m)
-       match (S m) with
-       | 0 => ss
-       | 1 => ss
-       | S (S n2) =>
-           if ltb h (n0 + length t0) then StageSet.add (S n2) ss else ss
-       end = true) as Ub1.
-    destruct m ; auto.
-    destruct (ltb h (n0 + length t0)) ; auto.
-    rewrite <- StageSetProperties.ub_le_1 ; auto.
-    specialize (H1 Ub1).
-    assert(StageSet.mem 0
-       match (S m) with
-       | 0 => ss
-       | 1 => ss
-       | S (S n2) =>
-           if ltb h (n0 + length t0) then StageSet.add (S n2) ss else ss
-       end = true) as P2.
-    destruct m ; auto.
-    destruct (ltb h (n0 + length t0)) ; auto.
-    rewrite StageSetProperties.add_mem_4 ; auto.
-    specialize (H1 P2).
-    inversion H1 ; subst.
-    apply eq_context_ssubst_ss_m_ge with (m:=0) ; auto ; omega.
-
-    destruct t1.
-    simpl in *|-*.
-    constructor ; auto.
-    apply eq_ssubst_context_ss_app ; auto.
-    specialize (H0 ss H2 H3).
-    apply eq_context_ssubst_ss_sum with (m1:=0) (b1:=(n0 + length t0)%nat) ; auto.
-    inversion H0 ; subst ; auto.
-
-    specialize (H1 ss H2 H3).
-    inversion H1 ; subst ; auto.
-
-    simpl in *|-* ; constructor ; auto.
-    apply eq_ssubst_context_ss_app ; auto.
-    specialize (H0 ss H2 H3).
-    inversion H0 ; subst ; auto.
-    apply eq_context_ssubst_ss_sum with (m1:=length t1) (b1:=(n0 + length t0)%nat) ; auto.
-    rewrite app_length ; omega.
-
-    specialize (H1 match (S m) with
-    | 0 => ss
-    | 1 => ss
-    | S (S n2) =>
-        if ltb h (n0 + length (t1 ++ t0)) then StageSet.add (S n2) ss else ss
-    end).
-    assert(StageSet.ub (S m)
-       match (S m) with
-       | 0 => ss
-       | 1 => ss
-       | S (S n2) =>
-           if ltb h (n0 + length (t1 ++ t0))
-           then StageSet.add (S n2) ss
-           else ss
-       end = true) as Ub1.
-    destruct m ; auto.
-    destruct (ltb h (n0 + length (t1 ++ t0))) ; auto.
-    rewrite <- StageSetProperties.ub_le_1 ; auto.
-    specialize (H1 Ub1).
-    assert(StageSet.mem 0
-       match (S m) with
-       | 0 => ss
-       | 1 => ss
-       | S (S n2) =>
-           if ltb h (n0 + length (t1 ++ t0))
-           then StageSet.add (S n2) ss
-           else ss
-       end = true) as P2.
-    destruct m ; auto.
-    destruct (ltb h (n0 + length (t1 ++ t0))) ; auto.
-    rewrite StageSetProperties.add_mem_4 ; auto.
-    specialize (H1 P2).
-    inversion H1 ; subst.
-    apply eq_context_ssubst_ss_m_ge with (m:=length t0) ; auto.
-    rewrite app_length ; omega.
-  Qed.
-
-  Lemma eq_ssubst_eq_strong:
+  Lemma eq_ssubst_2_ge:
     forall (e:S.expr) (bs:list nat) (h:S.var) (v:T.expr),
     let n := depth e in
     let (e0, cs) := trans e bs in
-    n < length bs ->
-    forall (ss:StageSet.t),
-    StageSet.ub n ss = true ->
-    (n > 0 -> (nth (pred n) bs 0 + booker e (pred n) <= h \/ StageSet.mem 0 ss = true)) ->
-    eq_ssubst_ss ss n h (booker e 0) v (nth 0 bs 0) e0 e0 /\
-    eq_stack_ssubst_ss (StageSet.remove n ss) (pred n) h v 
+    forall (m:nat), 
+    n <= m < length bs ->
+    eq_ssubst_2 m h (booker e 0) v (nth 0 bs 0) e0 e0 /\
+    eq_stack_ssubst_2 (pred m) h v 
                        (List.tl bs) (List.hd 0 bs) cs cs /\
-    (svalue 0 e -> eq_ssubst_ss ss n h (booker e 0) v (nth 0 bs 0) (phi e bs) (phi e bs)).
+    (svalue 0 e -> eq_ssubst_2 m h (booker e 0) v (nth 0 bs 0) (phi e bs) (phi e bs)).
   Proof.
     assert(forall (h v:nat), beq_nat (hole_var h) (source_var v) = false) as BeqFalse.
       intros ; apply beq_nat_false_iff ; unfold hole_var, source_var ; omega.
@@ -3834,1093 +4023,341 @@ Module TranslationProperties (R:Replacement)
     induction e ; simpl ; intros.
 
     (* EConst *)
-    unfold eq_ssubst_ss ; repeat(split) ; intros ;
+    unfold eq_ssubst_2 ; repeat(split) ; intros ;
     [rewrite MP.ssubst_ret | constructor |] ; 
     rewrite MP.ssubst_econst ; auto.
 
     
     (* EVar *)
-    unfold eq_ssubst_ss ; repeat(split) ; intros ;
+    unfold eq_ssubst_2 ; repeat(split) ; intros ;
     [rewrite MP.ssubst_ret | constructor |] ;
     rewrite MP.ssubst_evar, BeqFalse ; auto.
 
     (* EAbs *)
     specialize (IHe bs h v0) ;
     destruct (trans e) ; intros ;
-    unfold eq_ssubst_ss ; repeat(split) ; intros ;
-    destruct IHe with (ss:=ss) ; auto ; [
-    rewrite MP.ssubst_ret, MP.ssubst_eabs, BeqFalse, H2 |
-    destruct H3 | rewrite MP.ssubst_eabs, BeqFalse, H3 ] ; auto.
+    unfold eq_ssubst_2 ; repeat(split) ; intros ;
+    destruct IHe with (m:=m) ; auto ; [
+    rewrite MP.ssubst_ret, MP.ssubst_eabs, BeqFalse, H1 |
+    destruct H1 | rewrite MP.ssubst_eabs, BeqFalse, H2 ] ; auto.
 
     (* EFix *)
     specialize (IHe bs h v1) ;
     destruct (trans e) ; intros ;
-    unfold eq_ssubst_ss ; repeat(split) ; intros ;
-    destruct IHe with (ss:=ss) ; auto ; [
-    rewrite MP.ssubst_ret, MP.ssubst_efix, BeqFalse, BeqFalse ; simpl ; rewrite H2 |
-    destruct H3 | rewrite MP.ssubst_efix, BeqFalse, BeqFalse ; simpl ; rewrite H3 ] ; auto.
+    unfold eq_ssubst_2 ; repeat(split) ; intros ;
+    destruct IHe with (m:=m) ; auto ; [
+    rewrite MP.ssubst_ret, MP.ssubst_efix, BeqFalse, BeqFalse ; simpl ; rewrite H1 |
+    destruct H1 | rewrite MP.ssubst_efix, BeqFalse, BeqFalse ; simpl ; rewrite H2 ] ; auto.
     
     (* EApp *)
-    specialize (depth_length e1 (map_iter_booker e2 bs 0)) ; intros DpthLength1.
-    specialize (depth_length e2 bs) ; intros DpthLength2.
-    specialize (eq_ssubst_merge e1 e2 bs h v) ; intros EqMerge.
-    specialize (eq_ssubst_ss_merge e1 e2 bs h v) ; intros EqMergeSS.
-    specialize (eq_ssubst_gt e1 (map_iter_booker e2 bs 0)) ; intros EqSS1.
-    specialize (eq_ssubst_gt e2 bs) ; intros EqSS2.
+    specialize (eq_ssubst_2_merge e1 e2 bs h v) ; intros EqMerge.
     specialize (IHe1 (map_iter_booker e2 bs 0) h v) ;
     specialize (IHe2 bs h v) ;
     destruct (trans e1) ; destruct (trans e2) ; intros.
-    unfold eq_ssubst_ss ; repeat(split) ; intros.
+    unfold eq_ssubst_2 ; repeat(split) ; intros.
     assert(nth 0 (map_iter_booker e2 bs 0) 0 + booker e1 0 =
      nth 0 bs 0 + (booker e1 0 + booker e2 0))%nat as EqNth.
      unfold map_iter_booker.
      specialize (List2Properties.map_iter_nth_indep 
       (fun b n : nat => (b + booker e2 n)%nat) bs 0 0 0) ; intros Prop1.
       rewrite Prop1 ; auto ; simpl ; omega.
-
-     specialize (max_spec (depth e1) (depth e2)) ; intros Comp.
-
-     assert((nth 0 (map_iter_booker e2 bs 0) 0 + booker e1 0) = 
-        (nth 0 bs 0 + (booker e1 0 + booker e2 0)))%nat as Eq1.
-        unfold map_iter_booker.
-        specialize (List2Properties.map_iter_nth_indep (fun b n : nat => b + booker e2 n)%nat bs 0 0 0 0) ; intros Nth1.
-        simpl in Nth1 ; rewrite Nth1 ; auto ; omega.
-
-     destruct Comp ; destruct H2 ; [| inversion H2 ; subst ] ;
-     rewrite H3 in *|-*.
-
-      (* Case depth e1 < depth e2 *)
-      destruct IHe2 with (ss:=match depth e2 with
-          | 0 => ss | 1 => ss | S (S n) =>
-          if ltb h (nth 0 bs 0 + (booker e1 0 + booker e2 0))
-          then StageSet.add (S n) ss else ss end) ; auto ; intros.
-          destruct (depth e2) ; auto.
-          destruct n ; auto.
-          destruct (ltb h (nth 0 bs 0 + (booker e1 0 + booker e2 0))) ; auto.
-          rewrite <- StageSetProperties.ub_le_1 ; auto.
-          specialize (H1 H4) ; destruct H1 ; [left|right] ; auto ; try(omega).
-          destruct (depth e2) ; auto.
-          destruct n ; auto.
-          destruct (ltb h (nth 0 bs 0 + (booker e1 0 + booker e2 0))) ; auto.
-          rewrite StageSetProperties.add_mem_4 ; auto.
-
-      remember (CRaw.svalueb 0 e1) ; destruct b ; symmetry in Heqb.
+     remember (CRaw.svalueb 0 e1) ; destruct b ; symmetry in Heqb.
     
-        (* Case svalue 0 e1 *)
-        apply CalculusProperties.svalueb_iff in Heqb.
+      (* Case svalue 0 e1 *)
+      destruct H ; apply max_lub_iff in H ; auto ; destruct H.
+      destruct IHe1 with (m:=m) ; destruct IHe2 with (m:=m) ; auto.
+      unfold map_iter_booker ; rewrite List2Properties.length_map_iter ; auto.
+      rewrite MP.ssubst_bind with (f2:=(fun v2 : T.expr => cast_eapp (phi e1 (map_iter_booker e2 bs 0)) v2)).
+      destruct m ; [rewrite H5 ; auto|].
+      unfold eq_ssubst_2 in H5.
+      remember (ltb h (nth 0 bs 0 + booker e2 0)) ; 
+      destruct b ; symmetry in Heqb0.
+      assert(ltb h (nth 0 bs 0 + (booker e1 0 + booker e2 0))%nat = true) as LtbTrue.
+      apply leb_iff ; apply leb_iff in Heqb0 ; omega.
+      rewrite LtbTrue, H5 ; auto.
+      rewrite H5 ; auto.
+      destruct (ltb h (nth 0 bs 0 + (booker e1 0 + booker e2 0))) ; auto.
+      rewrite <- StageSetProperties.ub_le_1 ; auto.
+      intros ; apply CalculusProperties.svalueb_iff in Heqb.
+      rewrite MP.ssubst_eapp ; destruct H4.
+      destruct m ; [rewrite H7 ; auto|].
+      unfold eq_ssubst_2 in H7.
+      rewrite EqNth in H7 ; rewrite H7 ; auto.
 
-        unfold eq_ssubst_ss in H4.
-        rewrite MP.ssubst_bind with (f2:=(fun v2 : T.expr => cast_eapp (phi e1 (map_iter_booker e2 bs 0)) v2)) ; auto.
-        destruct (depth e2) ; [exfalso ; omega|].
-        destruct n ; try(rewrite H4 ; auto).
-        remember (ltb h (nth 0 bs 0 + (booker e1 0 + booker e2 0))).
-        destruct b ; symmetry in Heqb0.
-        destruct (ltb h (nth 0 bs 0 + booker e2 0)) ; try(rewrite H4 ; auto).
-        rewrite StageSetProperties.add_mem_1 in H4 ; auto.
-        rewrite H4 ; auto.
-        apply StageSetProperties.add_mem_3.
-        assert(ltb h (nth 0 bs 0 + booker e2 0) = false) as False1.
-        apply leb_iff_conv ; apply leb_iff_conv in Heqb0 ; omega.
-        rewrite False1 in H4 ; rewrite H4 ; auto.
-        
-        
-        intros ; rewrite MP.ssubst_eapp.
-        specialize (EqSS1 h v (depth e2)) ; simpl in EqSS1.
-        destruct EqSS1 ; auto ; try(omega).
-        split ; auto.
-        unfold map_iter_booker ; rewrite List2Properties.length_map_iter ; auto.
-        destruct H7 ; specialize (H8 Heqb).
-        unfold eq_ssubst in H8.
-        rewrite Eq1 in H8 ; rewrite H8 ; auto.
+      (* Case not svalue 0 e1 *)
+      destruct H ; apply max_lub_iff in H ; auto ; destruct H.
+      destruct IHe1 with (m:=m) ; destruct IHe2 with (m:=m) ; auto.
+      unfold map_iter_booker ; rewrite List2Properties.length_map_iter ; auto.
 
-        (* Case not svalue 0 e1 *)
-        rewrite MP.ssubst_bind with (f2:=(fun v1 : T.expr => bind e0 (fun v2 : T.expr => cast_eapp v1 v2))) ; auto.
-        specialize (EqSS1 h v (depth e2)) ; simpl in EqSS1.
-        destruct EqSS1 ; auto ; try(omega).
-        split ; auto.
-        unfold map_iter_booker ; rewrite List2Properties.length_map_iter ; auto.
-        unfold eq_ssubst in H6.
-        rewrite Eq1 in H6 ; rewrite H6 ; auto.
-
-        intros.
-        rewrite MP.ssubst_bind with (f2:=(fun v0 : T.expr => cast_eapp (ssubst (depth e2)
-        match (depth e2) with
+      rewrite MP.ssubst_bind with (f2:=(fun v1 : T.expr => bind e0 (fun v2 : T.expr => cast_eapp v1 v2))).
+      destruct m ; [rewrite H3 ; auto|].
+      unfold eq_ssubst_2 in H3.
+      rewrite EqNth in H3 ; rewrite H3 ; auto.
+      intros.
+      rewrite MP.ssubst_bind with (f2:=(fun v0 : T.expr => cast_eapp (ssubst m
+        match m with
         | 0 => ss
-        | 1 => ss
-        | S (S n) =>
+        | S n =>
             if ltb h (nth 0 bs 0 + (booker e1 0 + booker e2 0))
-            then StageSet.add (S n) ss
+            then StageSet.add n ss
             else ss
         end (cast_var (hole_var h)) v2 v) v0)).
-        unfold eq_ssubst_ss in H4.
-        destruct (depth e2) ; [exfalso ; omega|].
-        destruct n ; try(rewrite H4 ; auto).
-        remember (ltb h (nth 0 bs 0 + (booker e1 0 + booker e2 0))).
-        destruct b ; symmetry in Heqb0.
-        destruct (ltb h (nth 0 bs 0 + booker e2 0)) ; try(rewrite H4 ; auto).
-        rewrite StageSetProperties.add_mem_1 in H4 ; auto.
-        rewrite H4 ; auto.
-        apply StageSetProperties.add_mem_3.
-        assert(ltb h (nth 0 bs 0 + booker e2 0) = false) as False1.
-        apply leb_iff_conv ; apply leb_iff_conv in Heqb0 ; omega.
-        rewrite False1 in H4 ; rewrite H4 ; auto.
+      destruct m ; [rewrite H5 ; auto |].
+      unfold eq_ssubst_2 in H5.
+      remember (ltb h (nth 0 bs 0 + booker e2 0)) ; destruct b ;
+      symmetry in Heqb0.
+      assert(ltb h (nth 0 bs 0 + (booker e1 0 + booker e2 0)) = true) as LtbTrue.
+      apply leb_iff ; apply leb_iff in Heqb0 ; omega.
+      rewrite LtbTrue, H5 ; auto.
+      rewrite H5 ; auto.
+      destruct (ltb h (nth 0 bs 0 + (booker e1 0 + booker e2 0))) ; auto.
+      rewrite <- StageSetProperties.ub_le_1 ; auto.
+      intros ; rewrite MP.ssubst_eapp ; auto.
 
-        intros ; rewrite MP.ssubst_eapp ; auto.
-
-      (* Case depth e1 = depth e2 *)
-      clear H2 ; assert(H2:=H5) ; clear H5.
-      rewrite <- H2 in H3 ; rewrite H3 in *|-*.
-
-
-      destruct IHe1 with (ss:=match depth e2 with
-        | 0 => ss | 1 => ss | S (S n) =>
-        if ltb h (nth 0 bs 0 + (booker e1 0 + booker e2 0))
-        then StageSet.add (S n) ss else ss end) ; auto ; intros.
-        unfold map_iter_booker ; rewrite List2Properties.length_map_iter ; auto.
-        destruct (depth e2) ; auto.
-        destruct n ; auto.
-        destruct (ltb h (nth 0 bs 0 + (booker e1 0 + booker e2 0))) ; auto.
-        rewrite <- StageSetProperties.ub_le_1 ; auto ; omega.
-        specialize (H1 H4) ; destruct H1 ; [left|right] ; auto ; try(omega).
-        unfold map_iter_booker.
-        specialize (List2Properties.map_iter_nth_indep (fun b n : nat => b + booker e2 n)%nat bs (pred (depth e1)) 0 0 0) ; intros Nth1.
-        simpl in Nth1 ; rewrite Nth1 ; auto ; try(omega).
-        rewrite plus_0_r ; apply le_trans with (m:=(nth (pred (depth e1)) bs 0 +
-        (booker e1 (pred (depth e1)) + booker e2 (pred (depth e1))))%nat) ; omega.
-        destruct (depth e2) ; auto.
-        destruct n ; auto.
-        destruct (ltb h (nth 0 bs 0 + (booker e1 0 + booker e2 0))) ; auto.
-        rewrite StageSetProperties.add_mem_4 ; auto.
-
-      destruct IHe2 with (ss:=match depth e2 with
-          | 0 => ss | 1 => ss | S (S n) =>
-          if ltb h (nth 0 bs 0 + (booker e1 0 + booker e2 0))
-          then StageSet.add (S n) ss else ss end) ; auto ; intros ; try(omega).
-          rewrite <- H2 in *|-* ; 
-          destruct (depth e2) ; auto.
-          destruct n ; auto.
-          destruct (ltb h (nth 0 bs 0 + (booker e1 0 + booker e2 0))) ; auto.
-          rewrite <- StageSetProperties.ub_le_1 ; auto.
-          rewrite H2 in *|-*.
-          specialize (H1 H6) ; destruct H1 ; [left|right] ; auto ; try(omega).
-          destruct (depth e1) ; auto.
-          destruct n ; auto.
-          destruct (ltb h (nth 0 bs 0 + (booker e1 0 + booker e2 0))) ; auto.
-          rewrite StageSetProperties.add_mem_4 ; auto.
-
-      rewrite <- H2 in *|-*.
-      remember (CRaw.svalueb 0 e1) ; destruct b ; symmetry in Heqb.
-    
-        (* Case svalue 0 e1 *)
-        apply CalculusProperties.svalueb_iff in Heqb.
-
-        unfold eq_ssubst_ss in H6.
-        rewrite MP.ssubst_bind with (f2:=(fun v2 : T.expr => cast_eapp (phi e1 (map_iter_booker e2 bs 0)) v2)) ; auto.
-        destruct (depth e2) ; try(rewrite H6 ; auto).
-        destruct n ; try(rewrite H6 ; auto).
-        remember (ltb h (nth 0 bs 0 + (booker e1 0 + booker e2 0))).
-        destruct b ; symmetry in Heqb0.
-        destruct (ltb h (nth 0 bs 0 + booker e2 0)) ; try(rewrite H6 ; auto).
-        rewrite StageSetProperties.add_mem_1 in H6 ; auto.
-        rewrite H6 ; auto.
-        apply StageSetProperties.add_mem_3.
-        assert(ltb h (nth 0 bs 0 + booker e2 0) = false) as False1.
-        apply leb_iff_conv ; apply leb_iff_conv in Heqb0 ; omega.
-        rewrite False1 in H6 ; rewrite H6 ; auto.
-        
-        intros ; destruct H5 ; rewrite MP.ssubst_eapp.
-        unfold eq_ssubst_ss in H8 ; rewrite Eq1 in H8.
-        destruct (depth e2) ; try(rewrite H8 ; auto).
-        destruct n ; try(rewrite H8 ; auto).
-        remember (ltb h (nth 0 bs 0 + (booker e1 0 + booker e2 0))).
-        destruct b ; symmetry in Heqb0 ; try(rewrite H8 ; auto).
-        rewrite StageSetProperties.add_mem_1 in H8 ; auto.
-        rewrite H8 ; auto.
-        apply StageSetProperties.add_mem_3.
-
-        (* Case not svalue 0 e1 *)
-        rewrite MP.ssubst_bind with (f2:=(fun v1 : T.expr => bind e0 (fun v2 : T.expr => cast_eapp v1 v2))) ; auto.
-        
-        unfold eq_ssubst_ss in H4.
-        destruct (depth e2) ; try(rewrite H4 ; auto).
-        destruct n ; try(rewrite H4 ; auto).
-        rewrite Eq1 in H4.
-        remember (ltb h (nth 0 bs 0 + (booker e1 0 + booker e2 0)))%nat ;
-        destruct b ; symmetry in Heqb0 ; try(rewrite H4 ; auto).
-        rewrite StageSetProperties.add_mem_1 in H4 ; auto.
-        rewrite H4 ; auto.
-        apply StageSetProperties.add_mem_3.
-
-        intros.
-        rewrite MP.ssubst_bind with (f2:=(fun v0 : T.expr => cast_eapp (ssubst (depth e2)
-        match (depth e2) with
-        | 0 => ss
-        | 1 => ss
-        | S (S n) =>
-            if ltb h (nth 0 bs 0 + (booker e1 0 + booker e2 0))
-            then StageSet.add (S n) ss
-            else ss
-        end (cast_var (hole_var h)) v2 v) v0)).
-        unfold eq_ssubst_ss in H6.
-        destruct (depth e2) ; try(rewrite H6 ; auto).
-        destruct n ; try(rewrite H6 ; auto).
-        remember (ltb h (nth 0 bs 0 + (booker e1 0 + booker e2 0))).
-        destruct b ; symmetry in Heqb0.
-        destruct (ltb h (nth 0 bs 0 + booker e2 0)) ; try(rewrite H6 ; auto).
-        rewrite StageSetProperties.add_mem_1 in H6 ; auto.
-        rewrite H6 ; auto.
-        apply StageSetProperties.add_mem_3.
-        assert(ltb h (nth 0 bs 0 + booker e2 0) = false) as False1.
-        apply leb_iff_conv ; apply leb_iff_conv in Heqb0 ; omega.
-        rewrite False1 in H6 ; rewrite H6 ; auto.
-
-        intros ; rewrite MP.ssubst_eapp ; auto.
-
-      (* Case depth e2 < depth e1 *)
-      assert(depth e2 < depth e1).
-      omega.
-      rewrite H4 in *|-*.
-      clear H4 H5 ; assert(H4:=H6) ; clear H6 m.
-      rewrite H3 in *|-*.
-
-      destruct IHe1 with (ss:=match depth e1 with
-        | 0 => ss | 1 => ss | S (S n) =>
-        if ltb h (nth 0 bs 0 + (booker e1 0 + booker e2 0))
-        then StageSet.add (S n) ss else ss end) ; auto ; intros.
-        unfold map_iter_booker ; rewrite List2Properties.length_map_iter ; auto.
-        destruct (depth e1) ; auto.
-        destruct n ; auto.
-        destruct (ltb h (nth 0 bs 0 + (booker e1 0 + booker e2 0))) ; auto.
-        rewrite <- StageSetProperties.ub_le_1 ; auto.
-        specialize (H1 H5) ; destruct H1 ; [left|right] ; auto ; try(omega).
-        unfold map_iter_booker.
-        specialize (List2Properties.map_iter_nth_indep (fun b n : nat => b + booker e2 n)%nat bs (pred (depth e1)) 0 0 0) ; intros Nth1.
-        simpl in Nth1 ; rewrite Nth1 ; auto ; try(omega).
-        rewrite plus_0_r ; apply le_trans with (m:=(nth (pred (depth e1)) bs 0 +
-        (booker e1 (pred (depth e1)) + booker e2 (pred (depth e1))))%nat) ; omega.
-        destruct (depth e1) ; auto.
-        destruct n ; auto.
-        destruct (ltb h (nth 0 bs 0 + (booker e1 0 + booker e2 0))) ; auto.
-        rewrite StageSetProperties.add_mem_4 ; auto.
-
-      remember (CRaw.svalueb 0 e1) ; destruct b ; symmetry in Heqb.
-
-        (* Case svalue 0 e1 *)
-        apply CalculusProperties.svalueb_iff in Heqb.
-
-        rewrite MP.ssubst_bind with (f2:=(fun v2 : T.expr => cast_eapp (phi e1 (map_iter_booker e2 bs 0)) v2)) ; auto.
-
-        specialize (EqSS2 h v (depth e1)) ; simpl in EqSS2.
-        destruct EqSS2 ; auto ; try(omega).
-        unfold eq_ssubst in H7.
-        destruct (depth e1) ; [exfalso ; omega|].
-        destruct n ; try(rewrite H7 ; auto).
-        remember (ltb h (nth 0 bs 0 + (booker e1 0 + booker e2 0))).
-        destruct b ; symmetry in Heqb0.
-        destruct (ltb h (nth 0 bs 0 + booker e2 0)) ; try(rewrite H7 ; auto).
-        rewrite <- StageSetProperties.ub_le_1 ; auto.
-        assert(ltb h (nth 0 bs 0 + booker e2 0) = false) as False1.
-        apply leb_iff_conv ; apply leb_iff_conv in Heqb0 ; omega.
-        rewrite False1 in H7 ; rewrite H7 ; auto.
-
-        intros ; destruct H6 ; rewrite MP.ssubst_eapp.
-        unfold eq_ssubst_ss in H7 ; rewrite Eq1 in H7.
-        destruct (depth e1) ; [exfalso ; omega|].
-        destruct n ; try(rewrite H7 ; auto).
-        remember (ltb h (nth 0 bs 0 + (booker e1 0 + booker e2 0))).
-        destruct b ; symmetry in Heqb0 ; try(rewrite H7 ; auto).
-        rewrite StageSetProperties.add_mem_1 in H7 ; auto.
-        rewrite H7 ; auto.
-        apply StageSetProperties.add_mem_3.
-
-        (* Case not svalue 0 e1 *)
-        specialize (EqSS2 h v (depth e1)) ; simpl in EqSS2.
-        destruct EqSS2 ; auto ; try(omega).
-        rewrite MP.ssubst_bind with (f2:=(fun v1 : T.expr => bind e0 (fun v2 : T.expr => cast_eapp v1 v2))) ; auto.
-
-        unfold eq_ssubst_ss in H5.
-        destruct (depth e1) ; [exfalso ; omega|].
-        destruct n ; try(rewrite H5 ; auto).
-        rewrite Eq1 in H5.
-        remember (ltb h (nth 0 bs 0 + (booker e1 0 + booker e2 0)))%nat ;
-        destruct b ; symmetry in Heqb0 ; try(rewrite H5 ; auto).
-        rewrite StageSetProperties.add_mem_1 in H5 ; auto.
-        rewrite H5 ; auto.
-        apply StageSetProperties.add_mem_3.
-
-        intros.
-        rewrite MP.ssubst_bind with (f2:=(fun v0 : T.expr => cast_eapp (ssubst (depth e1)
-        match (depth e1) with
-        | 0 => ss
-        | 1 => ss
-        | S (S n) =>
-            if ltb h (nth 0 bs 0 + (booker e1 0 + booker e2 0))
-            then StageSet.add (S n) ss
-            else ss
-        end (cast_var (hole_var h)) v2 v) v0)).
-
-        unfold eq_ssubst in H7.
-        destruct (depth e1) ; [exfalso ; omega|].
-        destruct n ; try(rewrite H7 ; auto).
-        remember (ltb h (nth 0 bs 0 + (booker e1 0 + booker e2 0))).
-        destruct b ; symmetry in Heqb0.
-        destruct (ltb h (nth 0 bs 0 + booker e2 0)) ; try(rewrite H7 ; auto).
-        rewrite <- StageSetProperties.ub_le_1 ; auto.
-        assert(ltb h (nth 0 bs 0 + booker e2 0) = false) as False1.
-        apply leb_iff_conv ; apply leb_iff_conv in Heqb0 ; omega.
-        rewrite False1 in H7 ; rewrite H7 ; auto.
-
-        intros ; rewrite MP.ssubst_eapp ; auto.
-
-      (* Stack case *)
-      remember (max (depth e1) (depth e2)).
-      rewrite DpthLength1, DpthLength2 in Heqn.
-      destruct n.
-
-      destruct t0 ; destruct t ; simpl in *|-* ; try(exfalso ; omega).
-      constructor.
-      specialize (EqSS1 h v) ; specialize (EqSS2 h v).
-
-      destruct H1 ; try(omega).
-
-      (* Case not mem 0 ss *)
-      
-      apply eq_stack_ssubst_forall ; auto.
-      rewrite ContextStaticProperties.merge_length.
-      rewrite <- Heqn ; auto.
+      destruct H ; apply max_lub_iff in H ; destruct H.
+      destruct IHe1 with (m:=m) ; destruct IHe2 with (m:=m) ; auto.
+      unfold map_iter_booker ; rewrite List2Properties.length_map_iter ; auto.
+      destruct H5 ; destruct H3 ; clear H2 H4 H6 H7 IHe1 IHe2.
       apply EqMerge ; auto.
-
-        (* Left *)
-        specialize (max_spec (length t) (length t0)) ; intros ;
-        destruct H2 ; destruct H2 ; rewrite H3 in *|-*.
-        apply EqSS1 ; auto.
-        unfold map_iter_booker ; rewrite List2Properties.length_map_iter ;
-        rewrite DpthLength1 ; omega.
-        destruct t ; [constructor | simpl in *|-* ].
-        apply eq_stack_ssubst_ss_forall ; auto ; simpl ; try(omega).
-        intros ; simpl in *|-*.
-        destruct IHe1 with (ss:=ss0) ; auto.
-        unfold map_iter_booker ; rewrite List2Properties.length_map_iter ; omega.
-        rewrite DpthLength1 in *|-* ; inversion Heqn ; subst.
-        rewrite StageSetProperties.ub_le_2 with (m:=length t1) ; auto.
-        intros ; left ; auto.
-        
-        inversion Heqn ; subst ; unfold map_iter_booker.
-        specialize (List2Properties.map_iter_nth_indep 
-        (fun b n : nat => (b + booker e2 n)%nat) bs (pred (depth e1)) 0 0) ; intros Nth1.
-        simpl in Nth1 ; intros ; rewrite Nth1.
-        rewrite DpthLength1 ; simpl ; auto.
-        inversion Heqn ; subst.
-        rewrite plus_0_r in *|-* ; omega.
-        rewrite DpthLength1 ; omega.
-
-        inversion Heqn ; subst ; destruct H6 ; auto.
-        rewrite DpthLength1 in *|-*.
-        rewrite StageSetProperties.remove_equal in H6 ; auto.
-        apply StageSetProperties.ub_mem_1 with (m:=length t1) ; auto.
-        
-        (* Right *)
-        specialize (max_spec (length t0) (length t)) ; intros ;
-        destruct H2 ; destruct H2 ; rewrite max_comm in H3 ; rewrite H3 in *|-*.
-        apply EqSS2 ; auto.
-        rewrite DpthLength2 ; omega.
-        simpl in *|-*.
-        rewrite DpthLength2 in *|-* ; inversion Heqn ; subst.
-        apply eq_stack_ssubst_ss_forall ; auto ; simpl ; try(omega).
-        intros ; simpl in *|-*.
-        destruct IHe2 with (ss:=ss0) ; auto ; try(omega).
-        rewrite StageSetProperties.ub_le_2 with (m:=n) ; auto.
-        omega.
-        intros ; left ; auto.
-        rewrite <- H5 ; simpl ; omega.
-
-        destruct H7 ; auto.
-        rewrite <- H5 in *|-*.
-        rewrite StageSetProperties.remove_equal in H7 ; auto.
-        apply StageSetProperties.ub_mem_1 with (m:=n) ; auto.
-        simpl ; rewrite <- StageSetProperties.ub_S ; auto.
-
-      (* Case mem 0 ss *)
-      rewrite DpthLength1, DpthLength2 in *|-*.
-      apply EqMergeSS ; clear EqMerge ; try(omega) ; intros.
-
-        (* Left *)
-        specialize (max_spec (length t) (length t0)) ; intros ;
-        destruct H4 ; destruct H4 ; rewrite H5 in *|-*.
-        destruct EqSS1 with (m:=S n) ; try(omega).
-        unfold map_iter_booker ; rewrite List2Properties.length_map_iter ; omega.
-        apply eq_stack_ssubst_forall ; auto ; try(omega).
-        destruct H7 ; apply H7.
-
-        destruct t ; [exfalso ; simpl in *|-* ; omega|].
-        simpl in Heqn ; inversion Heqn ; subst.
-        destruct IHe1 with (ss:=ss0) ; auto.
-        simpl ; unfold map_iter_booker ; rewrite List2Properties.length_map_iter ; omega.
-        rewrite StageSetProperties.ub_le_2 with (m:=length t1) ; simpl ; auto.
-        destruct H7 ; auto.
-        rewrite StageSetProperties.remove_equal in H7 ; auto.
-        apply StageSetProperties.ub_mem_1 with (m:=length t1) ; auto.
-        
-        (* Right *)
-        specialize (max_spec (length t0) (length t)) ; intros ;
-        destruct H4 ; destruct H4 ; rewrite max_comm in H5 ; rewrite H5 in *|-*.
-        destruct EqSS2 with (m:=S n) ; try(omega).
-        apply eq_stack_ssubst_forall ; auto ; try(omega).
-        destruct H7 ; apply H7.
-
-        destruct t0 ; [exfalso ; simpl in *|-* ; omega|].
-        simpl in Heqn ; inversion Heqn ; subst.
-        destruct IHe2 with (ss:=ss0) ; auto.
-        rewrite StageSetProperties.ub_le_2 with (m:=length t1) ; simpl ; auto.
-        destruct H7 ; auto.
-        rewrite StageSetProperties.remove_equal in H7 ; auto.
-        apply StageSetProperties.ub_mem_1 with (m:=length t1) ; auto.
-
-        simpl ; rewrite <- StageSetProperties.ub_S ; auto.
-        rewrite StageSetProperties.remove_mem_1 ; auto.
-
-      (* Value case *)
-      inversion H2.
+      split ; auto.
+      apply max_lub_iff ; omega.
+      inversion H0.
 
     (* ELoc *)
-    unfold eq_ssubst_ss ; repeat(split) ; intros ;
+    unfold eq_ssubst_2 ; repeat(split) ; intros ;
     [rewrite MP.ssubst_ret | constructor |] ; 
     rewrite MP.ssubst_eloc ; auto.
 
     (* ERef *)
     specialize (IHe bs h v) ;
     destruct (trans e) ; intros ;
-    unfold eq_ssubst_ss ; repeat(split) ; intros ;
-    destruct IHe with (ss:=ss) ; auto.
+    unfold eq_ssubst_2 ; repeat(split) ; intros ;
+    destruct IHe with (m:=m) ; auto.
     rewrite MP.ssubst_bind with (f2:= (fun v0 : T.expr => cast_eref v0)) ; 
     intros.
-    rewrite H2 ; auto.
+    rewrite H1 ; auto.
     rewrite MP.ssubst_eref ; reflexivity.
-    destruct H3 ; auto.
-    inversion H2.
+    destruct H1 ; auto.
+    inversion H0.
 
     (* EDeref *)
     specialize (IHe bs h v) ;
     destruct (trans e) ; intros ;
-    unfold eq_ssubst_ss ; repeat(split) ; intros ;
-    destruct IHe with (ss:=ss) ; auto.
+    unfold eq_ssubst_2 ; repeat(split) ; intros ;
+    destruct IHe with (m:=m) ; auto.
     rewrite MP.ssubst_bind with (f2:= (fun v0 : T.expr => cast_ederef v0)) ; 
     intros.
-    rewrite H2 ; auto.
+    rewrite H1 ; auto.
     rewrite MP.ssubst_ederef ; reflexivity.
-    destruct H3 ; auto.
-    inversion H2.
+    destruct H1 ; auto.
+    inversion H0.
 
     (* EAssign *)
-    specialize (depth_length e1 (map_iter_booker e2 bs 0)) ; intros DpthLength1.
-    specialize (depth_length e2 bs) ; intros DpthLength2.
-    specialize (eq_ssubst_merge e1 e2 bs h v) ; intros EqMerge.
-    specialize (eq_ssubst_ss_merge e1 e2 bs h v) ; intros EqMergeSS.
-    specialize (eq_ssubst_gt e1 (map_iter_booker e2 bs 0)) ; intros EqSS1.
-    specialize (eq_ssubst_gt e2 bs) ; intros EqSS2.
+    specialize (eq_ssubst_2_merge e1 e2 bs h v) ; intros EqMerge.
     specialize (IHe1 (map_iter_booker e2 bs 0) h v) ;
     specialize (IHe2 bs h v) ;
     destruct (trans e1) ; destruct (trans e2) ; intros.
-    unfold eq_ssubst_ss ; repeat(split) ; intros.
+    unfold eq_ssubst_2 ; repeat(split) ; intros.
     assert(nth 0 (map_iter_booker e2 bs 0) 0 + booker e1 0 =
      nth 0 bs 0 + (booker e1 0 + booker e2 0))%nat as EqNth.
      unfold map_iter_booker.
      specialize (List2Properties.map_iter_nth_indep 
       (fun b n : nat => (b + booker e2 n)%nat) bs 0 0 0) ; intros Prop1.
       rewrite Prop1 ; auto ; simpl ; omega.
-
-     specialize (max_spec (depth e1) (depth e2)) ; intros Comp.
-
-     assert((nth 0 (map_iter_booker e2 bs 0) 0 + booker e1 0) = 
-        (nth 0 bs 0 + (booker e1 0 + booker e2 0)))%nat as Eq1.
-        unfold map_iter_booker.
-        specialize (List2Properties.map_iter_nth_indep (fun b n : nat => b + booker e2 n)%nat bs 0 0 0 0) ; intros Nth1.
-        simpl in Nth1 ; rewrite Nth1 ; auto ; omega.
-
-     destruct Comp ; destruct H2 ; [| inversion H2 ; subst ] ;
-     rewrite H3 in *|-*.
-
-      (* Case depth e1 < depth e2 *)
-      destruct IHe2 with (ss:=match depth e2 with
-          | 0 => ss | 1 => ss | S (S n) =>
-          if ltb h (nth 0 bs 0 + (booker e1 0 + booker e2 0))
-          then StageSet.add (S n) ss else ss end) ; auto ; intros.
-          destruct (depth e2) ; auto.
-          destruct n ; auto.
-          destruct (ltb h (nth 0 bs 0 + (booker e1 0 + booker e2 0))) ; auto.
-          rewrite <- StageSetProperties.ub_le_1 ; auto.
-          specialize (H1 H4) ; destruct H1 ; [left|right] ; auto ; try(omega).
-          destruct (depth e2) ; auto.
-          destruct n ; auto.
-          destruct (ltb h (nth 0 bs 0 + (booker e1 0 + booker e2 0))) ; auto.
-          rewrite StageSetProperties.add_mem_4 ; auto.
-
-      remember (CRaw.svalueb 0 e1) ; destruct b ; symmetry in Heqb.
+     remember (CRaw.svalueb 0 e1) ; destruct b ; symmetry in Heqb.
     
-        (* Case svalue 0 e1 *)
-        apply CalculusProperties.svalueb_iff in Heqb.
+      (* Case svalue 0 e1 *)
+      destruct H ; apply max_lub_iff in H ; auto ; destruct H.
+      destruct IHe1 with (m:=m) ; destruct IHe2 with (m:=m) ; auto.
+      unfold map_iter_booker ; rewrite List2Properties.length_map_iter ; auto.
+      rewrite MP.ssubst_bind with (f2:=(fun v2 : T.expr => cast_eassign (phi e1 (map_iter_booker e2 bs 0)) v2)).
+      destruct m ; [rewrite H5 ; auto|].
+      unfold eq_ssubst_2 in H5.
+      remember (ltb h (nth 0 bs 0 + booker e2 0)) ; 
+      destruct b ; symmetry in Heqb0.
+      assert(ltb h (nth 0 bs 0 + (booker e1 0 + booker e2 0))%nat = true) as LtbTrue.
+      apply leb_iff ; apply leb_iff in Heqb0 ; omega.
+      rewrite LtbTrue, H5 ; auto.
+      rewrite H5 ; auto.
+      destruct (ltb h (nth 0 bs 0 + (booker e1 0 + booker e2 0))) ; auto.
+      rewrite <- StageSetProperties.ub_le_1 ; auto.
+      intros ; apply CalculusProperties.svalueb_iff in Heqb.
+      rewrite MP.ssubst_eassign ; destruct H4.
+      destruct m ; [rewrite H7 ; auto|].
+      unfold eq_ssubst_2 in H7.
+      rewrite EqNth in H7 ; rewrite H7 ; auto.
 
-        unfold eq_ssubst_ss in H4.
-        rewrite MP.ssubst_bind with (f2:=(fun v2 : T.expr => cast_eassign (phi e1 (map_iter_booker e2 bs 0)) v2)) ; auto.
-        destruct (depth e2) ; [exfalso ; omega|].
-        destruct n ; try(rewrite H4 ; auto).
-        remember (ltb h (nth 0 bs 0 + (booker e1 0 + booker e2 0))).
-        destruct b ; symmetry in Heqb0.
-        destruct (ltb h (nth 0 bs 0 + booker e2 0)) ; try(rewrite H4 ; auto).
-        rewrite StageSetProperties.add_mem_1 in H4 ; auto.
-        rewrite H4 ; auto.
-        apply StageSetProperties.add_mem_3.
-        assert(ltb h (nth 0 bs 0 + booker e2 0) = false) as False1.
-        apply leb_iff_conv ; apply leb_iff_conv in Heqb0 ; omega.
-        rewrite False1 in H4 ; rewrite H4 ; auto.
-        
-        
-        intros ; rewrite MP.ssubst_eassign.
-        specialize (EqSS1 h v (depth e2)) ; simpl in EqSS1.
-        destruct EqSS1 ; auto ; try(omega).
-        split ; auto.
-        unfold map_iter_booker ; rewrite List2Properties.length_map_iter ; auto.
-        destruct H7 ; specialize (H8 Heqb).
-        unfold eq_ssubst in H8.
-        rewrite Eq1 in H8 ; rewrite H8 ; auto.
+      (* Case not svalue 0 e1 *)
+      destruct H ; apply max_lub_iff in H ; auto ; destruct H.
+      destruct IHe1 with (m:=m) ; destruct IHe2 with (m:=m) ; auto.
+      unfold map_iter_booker ; rewrite List2Properties.length_map_iter ; auto.
 
-        (* Case not svalue 0 e1 *)
-        rewrite MP.ssubst_bind with (f2:=(fun v1 : T.expr => bind e0 (fun v2 : T.expr => cast_eassign v1 v2))) ; auto.
-        specialize (EqSS1 h v (depth e2)) ; simpl in EqSS1.
-        destruct EqSS1 ; auto ; try(omega).
-        split ; auto.
-        unfold map_iter_booker ; rewrite List2Properties.length_map_iter ; auto.
-        unfold eq_ssubst in H6.
-        rewrite Eq1 in H6 ; rewrite H6 ; auto.
-
-        intros.
-        rewrite MP.ssubst_bind with (f2:=(fun v0 : T.expr => cast_eassign (ssubst (depth e2)
-        match (depth e2) with
+      rewrite MP.ssubst_bind with (f2:=(fun v1 : T.expr => bind e0 (fun v2 : T.expr => cast_eassign v1 v2))).
+      destruct m ; [rewrite H3 ; auto|].
+      unfold eq_ssubst_2 in H3.
+      rewrite EqNth in H3 ; rewrite H3 ; auto.
+      intros.
+      rewrite MP.ssubst_bind with (f2:=(fun v0 : T.expr => cast_eassign (ssubst m
+        match m with
         | 0 => ss
-        | 1 => ss
-        | S (S n) =>
+        | S n =>
             if ltb h (nth 0 bs 0 + (booker e1 0 + booker e2 0))
-            then StageSet.add (S n) ss
+            then StageSet.add n ss
             else ss
         end (cast_var (hole_var h)) v2 v) v0)).
-        unfold eq_ssubst_ss in H4.
-        destruct (depth e2) ; [exfalso ; omega|].
-        destruct n ; try(rewrite H4 ; auto).
-        remember (ltb h (nth 0 bs 0 + (booker e1 0 + booker e2 0))).
-        destruct b ; symmetry in Heqb0.
-        destruct (ltb h (nth 0 bs 0 + booker e2 0)) ; try(rewrite H4 ; auto).
-        rewrite StageSetProperties.add_mem_1 in H4 ; auto.
-        rewrite H4 ; auto.
-        apply StageSetProperties.add_mem_3.
-        assert(ltb h (nth 0 bs 0 + booker e2 0) = false) as False1.
-        apply leb_iff_conv ; apply leb_iff_conv in Heqb0 ; omega.
-        rewrite False1 in H4 ; rewrite H4 ; auto.
+      destruct m ; [rewrite H5 ; auto |].
+      unfold eq_ssubst_2 in H5.
+      remember (ltb h (nth 0 bs 0 + booker e2 0)) ; destruct b ;
+      symmetry in Heqb0.
+      assert(ltb h (nth 0 bs 0 + (booker e1 0 + booker e2 0)) = true) as LtbTrue.
+      apply leb_iff ; apply leb_iff in Heqb0 ; omega.
+      rewrite LtbTrue, H5 ; auto.
+      rewrite H5 ; auto.
+      destruct (ltb h (nth 0 bs 0 + (booker e1 0 + booker e2 0))) ; auto.
+      rewrite <- StageSetProperties.ub_le_1 ; auto.
+      intros ; rewrite MP.ssubst_eassign ; auto.
 
-        intros ; rewrite MP.ssubst_eassign ; auto.
-
-      (* Case depth e1 = depth e2 *)
-      clear H2 ; assert(H2:=H5) ; clear H5.
-      rewrite <- H2 in H3 ; rewrite H3 in *|-*.
-
-
-      destruct IHe1 with (ss:=match depth e2 with
-        | 0 => ss | 1 => ss | S (S n) =>
-        if ltb h (nth 0 bs 0 + (booker e1 0 + booker e2 0))
-        then StageSet.add (S n) ss else ss end) ; auto ; intros.
-        unfold map_iter_booker ; rewrite List2Properties.length_map_iter ; auto.
-        destruct (depth e2) ; auto.
-        destruct n ; auto.
-        destruct (ltb h (nth 0 bs 0 + (booker e1 0 + booker e2 0))) ; auto.
-        rewrite <- StageSetProperties.ub_le_1 ; auto ; omega.
-        specialize (H1 H4) ; destruct H1 ; [left|right] ; auto ; try(omega).
-        unfold map_iter_booker.
-        specialize (List2Properties.map_iter_nth_indep (fun b n : nat => b + booker e2 n)%nat bs (pred (depth e1)) 0 0 0) ; intros Nth1.
-        simpl in Nth1 ; rewrite Nth1 ; auto ; try(omega).
-        rewrite plus_0_r ; apply le_trans with (m:=(nth (pred (depth e1)) bs 0 +
-        (booker e1 (pred (depth e1)) + booker e2 (pred (depth e1))))%nat) ; omega.
-        destruct (depth e2) ; auto.
-        destruct n ; auto.
-        destruct (ltb h (nth 0 bs 0 + (booker e1 0 + booker e2 0))) ; auto.
-        rewrite StageSetProperties.add_mem_4 ; auto.
-
-      destruct IHe2 with (ss:=match depth e2 with
-          | 0 => ss | 1 => ss | S (S n) =>
-          if ltb h (nth 0 bs 0 + (booker e1 0 + booker e2 0))
-          then StageSet.add (S n) ss else ss end) ; auto ; intros ; try(omega).
-          rewrite <- H2 in *|-* ; 
-          destruct (depth e2) ; auto.
-          destruct n ; auto.
-          destruct (ltb h (nth 0 bs 0 + (booker e1 0 + booker e2 0))) ; auto.
-          rewrite <- StageSetProperties.ub_le_1 ; auto.
-          rewrite H2 in *|-*.
-          specialize (H1 H6) ; destruct H1 ; [left|right] ; auto ; try(omega).
-          destruct (depth e1) ; auto.
-          destruct n ; auto.
-          destruct (ltb h (nth 0 bs 0 + (booker e1 0 + booker e2 0))) ; auto.
-          rewrite StageSetProperties.add_mem_4 ; auto.
-
-      rewrite <- H2 in *|-*.
-      remember (CRaw.svalueb 0 e1) ; destruct b ; symmetry in Heqb.
-    
-        (* Case svalue 0 e1 *)
-        apply CalculusProperties.svalueb_iff in Heqb.
-
-        unfold eq_ssubst_ss in H6.
-        rewrite MP.ssubst_bind with (f2:=(fun v2 : T.expr => cast_eassign (phi e1 (map_iter_booker e2 bs 0)) v2)) ; auto.
-        destruct (depth e2) ; try(rewrite H6 ; auto).
-        destruct n ; try(rewrite H6 ; auto).
-        remember (ltb h (nth 0 bs 0 + (booker e1 0 + booker e2 0))).
-        destruct b ; symmetry in Heqb0.
-        destruct (ltb h (nth 0 bs 0 + booker e2 0)) ; try(rewrite H6 ; auto).
-        rewrite StageSetProperties.add_mem_1 in H6 ; auto.
-        rewrite H6 ; auto.
-        apply StageSetProperties.add_mem_3.
-        assert(ltb h (nth 0 bs 0 + booker e2 0) = false) as False1.
-        apply leb_iff_conv ; apply leb_iff_conv in Heqb0 ; omega.
-        rewrite False1 in H6 ; rewrite H6 ; auto.
-        
-        intros ; destruct H5 ; rewrite MP.ssubst_eassign.
-        unfold eq_ssubst_ss in H8 ; rewrite Eq1 in H8.
-        destruct (depth e2) ; try(rewrite H8 ; auto).
-        destruct n ; try(rewrite H8 ; auto).
-        remember (ltb h (nth 0 bs 0 + (booker e1 0 + booker e2 0))).
-        destruct b ; symmetry in Heqb0 ; try(rewrite H8 ; auto).
-        rewrite StageSetProperties.add_mem_1 in H8 ; auto.
-        rewrite H8 ; auto.
-        apply StageSetProperties.add_mem_3.
-
-        (* Case not svalue 0 e1 *)
-        rewrite MP.ssubst_bind with (f2:=(fun v1 : T.expr => bind e0 (fun v2 : T.expr => cast_eassign v1 v2))) ; auto.
-        
-        unfold eq_ssubst_ss in H4.
-        destruct (depth e2) ; try(rewrite H4 ; auto).
-        destruct n ; try(rewrite H4 ; auto).
-        rewrite Eq1 in H4.
-        remember (ltb h (nth 0 bs 0 + (booker e1 0 + booker e2 0)))%nat ;
-        destruct b ; symmetry in Heqb0 ; try(rewrite H4 ; auto).
-        rewrite StageSetProperties.add_mem_1 in H4 ; auto.
-        rewrite H4 ; auto.
-        apply StageSetProperties.add_mem_3.
-
-        intros.
-        rewrite MP.ssubst_bind with (f2:=(fun v0 : T.expr => cast_eassign (ssubst (depth e2)
-        match (depth e2) with
-        | 0 => ss
-        | 1 => ss
-        | S (S n) =>
-            if ltb h (nth 0 bs 0 + (booker e1 0 + booker e2 0))
-            then StageSet.add (S n) ss
-            else ss
-        end (cast_var (hole_var h)) v2 v) v0)).
-        unfold eq_ssubst_ss in H6.
-        destruct (depth e2) ; try(rewrite H6 ; auto).
-        destruct n ; try(rewrite H6 ; auto).
-        remember (ltb h (nth 0 bs 0 + (booker e1 0 + booker e2 0))).
-        destruct b ; symmetry in Heqb0.
-        destruct (ltb h (nth 0 bs 0 + booker e2 0)) ; try(rewrite H6 ; auto).
-        rewrite StageSetProperties.add_mem_1 in H6 ; auto.
-        rewrite H6 ; auto.
-        apply StageSetProperties.add_mem_3.
-        assert(ltb h (nth 0 bs 0 + booker e2 0) = false) as False1.
-        apply leb_iff_conv ; apply leb_iff_conv in Heqb0 ; omega.
-        rewrite False1 in H6 ; rewrite H6 ; auto.
-
-        intros ; rewrite MP.ssubst_eassign ; auto.
-
-      (* Case depth e2 < depth e1 *)
-      assert(depth e2 < depth e1).
-      omega.
-      rewrite H4 in *|-*.
-      clear H4 H5 ; assert(H4:=H6) ; clear H6 m.
-      rewrite H3 in *|-*.
-
-      destruct IHe1 with (ss:=match depth e1 with
-        | 0 => ss | 1 => ss | S (S n) =>
-        if ltb h (nth 0 bs 0 + (booker e1 0 + booker e2 0))
-        then StageSet.add (S n) ss else ss end) ; auto ; intros.
-        unfold map_iter_booker ; rewrite List2Properties.length_map_iter ; auto.
-        destruct (depth e1) ; auto.
-        destruct n ; auto.
-        destruct (ltb h (nth 0 bs 0 + (booker e1 0 + booker e2 0))) ; auto.
-        rewrite <- StageSetProperties.ub_le_1 ; auto.
-        specialize (H1 H5) ; destruct H1 ; [left|right] ; auto ; try(omega).
-        unfold map_iter_booker.
-        specialize (List2Properties.map_iter_nth_indep (fun b n : nat => b + booker e2 n)%nat bs (pred (depth e1)) 0 0 0) ; intros Nth1.
-        simpl in Nth1 ; rewrite Nth1 ; auto ; try(omega).
-        rewrite plus_0_r ; apply le_trans with (m:=(nth (pred (depth e1)) bs 0 +
-        (booker e1 (pred (depth e1)) + booker e2 (pred (depth e1))))%nat) ; omega.
-        destruct (depth e1) ; auto.
-        destruct n ; auto.
-        destruct (ltb h (nth 0 bs 0 + (booker e1 0 + booker e2 0))) ; auto.
-        rewrite StageSetProperties.add_mem_4 ; auto.
-
-      remember (CRaw.svalueb 0 e1) ; destruct b ; symmetry in Heqb.
-
-        (* Case svalue 0 e1 *)
-        apply CalculusProperties.svalueb_iff in Heqb.
-
-        rewrite MP.ssubst_bind with (f2:=(fun v2 : T.expr => cast_eassign (phi e1 (map_iter_booker e2 bs 0)) v2)) ; auto.
-
-        specialize (EqSS2 h v (depth e1)) ; simpl in EqSS2.
-        destruct EqSS2 ; auto ; try(omega).
-        unfold eq_ssubst in H7.
-        destruct (depth e1) ; [exfalso ; omega|].
-        destruct n ; try(rewrite H7 ; auto).
-        remember (ltb h (nth 0 bs 0 + (booker e1 0 + booker e2 0))).
-        destruct b ; symmetry in Heqb0.
-        destruct (ltb h (nth 0 bs 0 + booker e2 0)) ; try(rewrite H7 ; auto).
-        rewrite <- StageSetProperties.ub_le_1 ; auto.
-        assert(ltb h (nth 0 bs 0 + booker e2 0) = false) as False1.
-        apply leb_iff_conv ; apply leb_iff_conv in Heqb0 ; omega.
-        rewrite False1 in H7 ; rewrite H7 ; auto.
-
-        intros ; destruct H6 ; rewrite MP.ssubst_eassign.
-        unfold eq_ssubst_ss in H7 ; rewrite Eq1 in H7.
-        destruct (depth e1) ; [exfalso ; omega|].
-        destruct n ; try(rewrite H7 ; auto).
-        remember (ltb h (nth 0 bs 0 + (booker e1 0 + booker e2 0))).
-        destruct b ; symmetry in Heqb0 ; try(rewrite H7 ; auto).
-        rewrite StageSetProperties.add_mem_1 in H7 ; auto.
-        rewrite H7 ; auto.
-        apply StageSetProperties.add_mem_3.
-
-        (* Case not svalue 0 e1 *)
-        specialize (EqSS2 h v (depth e1)) ; simpl in EqSS2.
-        destruct EqSS2 ; auto ; try(omega).
-        rewrite MP.ssubst_bind with (f2:=(fun v1 : T.expr => bind e0 (fun v2 : T.expr => cast_eassign v1 v2))) ; auto.
-
-        unfold eq_ssubst_ss in H5.
-        destruct (depth e1) ; [exfalso ; omega|].
-        destruct n ; try(rewrite H5 ; auto).
-        rewrite Eq1 in H5.
-        remember (ltb h (nth 0 bs 0 + (booker e1 0 + booker e2 0)))%nat ;
-        destruct b ; symmetry in Heqb0 ; try(rewrite H5 ; auto).
-        rewrite StageSetProperties.add_mem_1 in H5 ; auto.
-        rewrite H5 ; auto.
-        apply StageSetProperties.add_mem_3.
-
-        intros.
-        rewrite MP.ssubst_bind with (f2:=(fun v0 : T.expr => cast_eassign (ssubst (depth e1)
-        match (depth e1) with
-        | 0 => ss
-        | 1 => ss
-        | S (S n) =>
-            if ltb h (nth 0 bs 0 + (booker e1 0 + booker e2 0))
-            then StageSet.add (S n) ss
-            else ss
-        end (cast_var (hole_var h)) v2 v) v0)).
-
-        unfold eq_ssubst in H7.
-        destruct (depth e1) ; [exfalso ; omega|].
-        destruct n ; try(rewrite H7 ; auto).
-        remember (ltb h (nth 0 bs 0 + (booker e1 0 + booker e2 0))).
-        destruct b ; symmetry in Heqb0.
-        destruct (ltb h (nth 0 bs 0 + booker e2 0)) ; try(rewrite H7 ; auto).
-        rewrite <- StageSetProperties.ub_le_1 ; auto.
-        assert(ltb h (nth 0 bs 0 + booker e2 0) = false) as False1.
-        apply leb_iff_conv ; apply leb_iff_conv in Heqb0 ; omega.
-        rewrite False1 in H7 ; rewrite H7 ; auto.
-
-        intros ; rewrite MP.ssubst_eassign ; auto.
-
-      (* Stack case *)
-      remember (max (depth e1) (depth e2)).
-      rewrite DpthLength1, DpthLength2 in Heqn.
-      destruct n.
-
-      destruct t0 ; destruct t ; simpl in *|-* ; try(exfalso ; omega).
-      constructor.
-      specialize (EqSS1 h v) ; specialize (EqSS2 h v).
-
-      destruct H1 ; try(omega).
-
-      (* Case not mem 0 ss *)
-      
-      apply eq_stack_ssubst_forall ; auto.
-      rewrite ContextStaticProperties.merge_length.
-      rewrite <- Heqn ; auto.
+      destruct H ; apply max_lub_iff in H ; destruct H.
+      destruct IHe1 with (m:=m) ; destruct IHe2 with (m:=m) ; auto.
+      unfold map_iter_booker ; rewrite List2Properties.length_map_iter ; auto.
+      destruct H5 ; destruct H3.
       apply EqMerge ; auto.
-
-        (* Left *)
-        specialize (max_spec (length t) (length t0)) ; intros ;
-        destruct H2 ; destruct H2 ; rewrite H3 in *|-*.
-        apply EqSS1 ; auto.
-        unfold map_iter_booker ; rewrite List2Properties.length_map_iter ;
-        rewrite DpthLength1 ; omega.
-        destruct t ; [constructor | simpl in *|-* ].
-        apply eq_stack_ssubst_ss_forall ; auto ; simpl ; try(omega).
-        intros ; simpl in *|-*.
-        destruct IHe1 with (ss:=ss0) ; auto.
-        unfold map_iter_booker ; rewrite List2Properties.length_map_iter ; omega.
-        rewrite DpthLength1 in *|-* ; inversion Heqn ; subst.
-        rewrite StageSetProperties.ub_le_2 with (m:=length t1) ; auto.
-        intros ; left ; auto.
-        
-        inversion Heqn ; subst ; unfold map_iter_booker.
-        specialize (List2Properties.map_iter_nth_indep 
-        (fun b n : nat => (b + booker e2 n)%nat) bs (pred (depth e1)) 0 0) ; intros Nth1.
-        simpl in Nth1 ; intros ; rewrite Nth1.
-        rewrite DpthLength1 ; simpl ; auto.
-        inversion Heqn ; subst.
-        rewrite plus_0_r in *|-* ; omega.
-        rewrite DpthLength1 ; omega.
-
-        inversion Heqn ; subst ; destruct H6 ; auto.
-        rewrite DpthLength1 in *|-*.
-        rewrite StageSetProperties.remove_equal in H6 ; auto.
-        apply StageSetProperties.ub_mem_1 with (m:=length t1) ; auto.
-        
-        (* Right *)
-        specialize (max_spec (length t0) (length t)) ; intros ;
-        destruct H2 ; destruct H2 ; rewrite max_comm in H3 ; rewrite H3 in *|-*.
-        apply EqSS2 ; auto.
-        rewrite DpthLength2 ; omega.
-        simpl in *|-*.
-        rewrite DpthLength2 in *|-* ; inversion Heqn ; subst.
-        apply eq_stack_ssubst_ss_forall ; auto ; simpl ; try(omega).
-        intros ; simpl in *|-*.
-        destruct IHe2 with (ss:=ss0) ; auto ; try(omega).
-        rewrite StageSetProperties.ub_le_2 with (m:=n) ; auto.
-        omega.
-        intros ; left ; auto.
-        rewrite <- H5 ; simpl ; omega.
-
-        destruct H7 ; auto.
-        rewrite <- H5 in *|-*.
-        rewrite StageSetProperties.remove_equal in H7 ; auto.
-        apply StageSetProperties.ub_mem_1 with (m:=n) ; auto.
-        simpl ; rewrite <- StageSetProperties.ub_S ; auto.
-
-      (* Case mem 0 ss *)
-      rewrite DpthLength1, DpthLength2 in *|-*.
-      apply EqMergeSS ; clear EqMerge ; try(omega) ; intros.
-
-        (* Left *)
-        specialize (max_spec (length t) (length t0)) ; intros ;
-        destruct H4 ; destruct H4 ; rewrite H5 in *|-*.
-        destruct EqSS1 with (m:=S n) ; try(omega).
-        unfold map_iter_booker ; rewrite List2Properties.length_map_iter ; omega.
-        apply eq_stack_ssubst_forall ; auto ; try(omega).
-        destruct H7 ; apply H7.
-
-        destruct t ; [exfalso ; simpl in *|-* ; omega|].
-        simpl in Heqn ; inversion Heqn ; subst.
-        destruct IHe1 with (ss:=ss0) ; auto.
-        simpl ; unfold map_iter_booker ; rewrite List2Properties.length_map_iter ; omega.
-        rewrite StageSetProperties.ub_le_2 with (m:=length t1) ; simpl ; auto.
-        destruct H7 ; auto.
-        rewrite StageSetProperties.remove_equal in H7 ; auto.
-        apply StageSetProperties.ub_mem_1 with (m:=length t1) ; auto.
-        
-        (* Right *)
-        specialize (max_spec (length t0) (length t)) ; intros ;
-        destruct H4 ; destruct H4 ; rewrite max_comm in H5 ; rewrite H5 in *|-*.
-        destruct EqSS2 with (m:=S n) ; try(omega).
-        apply eq_stack_ssubst_forall ; auto ; try(omega).
-        destruct H7 ; apply H7.
-
-        destruct t0 ; [exfalso ; simpl in *|-* ; omega|].
-        simpl in Heqn ; inversion Heqn ; subst.
-        destruct IHe2 with (ss:=ss0) ; auto.
-        rewrite StageSetProperties.ub_le_2 with (m:=length t1) ; simpl ; auto.
-        destruct H7 ; auto.
-        rewrite StageSetProperties.remove_equal in H7 ; auto.
-        apply StageSetProperties.ub_mem_1 with (m:=length t1) ; auto.
-
-        simpl ; rewrite <- StageSetProperties.ub_S ; auto.
-        rewrite StageSetProperties.remove_mem_1 ; auto.
-
-      (* Value case *)
-      inversion H2.
+      split ; auto.
+      apply max_lub_iff ; omega.
+      inversion H0.
 
     (* EBox *)
     specialize (IHe (0::bs) h v) ;
     specialize (booker_length e (0::bs)) ; intros BKLength.
     specialize (depth_length e (0::bs)) ; intros DpthLength1.
-    specialize (eq_ssubst_gt e (0::bs)) ; intros EqGt.
-    specialize (eq_ssubst_fill_eq_1 e bs) ; intros EqFill1.
-    specialize (eq_ssubst_fill_eq_2 e bs) ; intros EqFill2.
-    specialize (eq_ssubst_fill_eq_3 e bs) ; intros EqFill3.
+    specialize (eq_ssubst_2_fill_ge_1 e bs) ; intros EqFill1.
+    specialize (eq_ssubst_2_fill_ge_2 e bs) ; intros EqFill2.
     destruct (trans e) ; intros.
-    destruct t ; simpl in *|-* ; intros ;
-    rewrite BKLength in *|-* ; rewrite DpthLength1 in *|-* ; simpl in *|-*.
+    destruct t ; simpl in *|-* ; intros.
 
       (* depth e = 0 *)
-      destruct EqGt with (h:=h) (v:=v) (m:=1) ; auto.
-      omega.
-      unfold eq_ssubst_ss ; repeat(split) ; intros.
-      rewrite MP.ssubst_ret, MP.ssubst_ebox.
-      rewrite H2 ; auto.
-      rewrite StageSetProperties.ub_le_2 with (m:=0) ; auto.
+      unfold eq_ssubst_2 ; repeat(split) ; intros.
+
+      rewrite MP.ssubst_ret, MP.ssubst_ebox ;
+      rewrite DpthLength1 in *|-* ;
+      rewrite BKLength in *|-* ; simpl in *|-* ;
+      destruct IHe with (m:=S m) ; auto ; try(omega).
+      unfold eq_ssubst_2 in H1 ; simpl in H1 ;
+      destruct m ; rewrite H1 ; auto ; [
+      rewrite StageSetProperties.ub_le_2 with (m:=0) ; auto | ] ;
+      destruct m ; auto ; destruct (ltb h (nth 0 bs 0 + 0)) ; auto ;
+      try(rewrite <- StageSetProperties.ub_le_1 ; auto) ;
+      try(apply StageSetProperties.ub_le_2 with (m:=(S (S m))) ; auto) ;
+      try(rewrite StageSetProperties.ub_le_2 with (m:=1) ; auto ; omega).
+
       constructor.
-      rewrite MP.ssubst_ebox.
-      rewrite H2 ; auto.
-      rewrite StageSetProperties.ub_le_2 with (m:=0) ; auto.
 
-      (* depth e = 1 *)
-      destruct t0 ; intros ; simpl in *|-*.
-      remember (ltb h ((length t))%nat).
-      symmetry in Heqb ; destruct b.
-      destruct IHe with (ss:=(StageSet.add 0 ss)) ; auto ; try(omega).
-      rewrite <- StageSetProperties.ub_le_1 ; auto.
-      rewrite StageSetProperties.ub_le_2 with (m:=0) ; auto.
-      intros ; right ; apply StageSetProperties.add_mem_3 ; auto.
+      rewrite MP.ssubst_ebox ;
+      rewrite DpthLength1 in *|-* ;
+      rewrite BKLength in *|-* ; simpl in *|-* ;
+      destruct IHe with (m:=S m) ; auto ; try(omega) ;
+      unfold eq_ssubst_2 in H2 ; simpl in H2 ;
+      destruct m ; rewrite H2 ; auto ; [
+      rewrite StageSetProperties.ub_le_2 with (m:=0) ; auto | ] ;
+      destruct m ; auto ; destruct (ltb h (nth 0 bs 0 + 0)) ; auto ;
+      try(rewrite <- StageSetProperties.ub_le_1 ; auto) ;
+      try(apply StageSetProperties.ub_le_2 with (m:=(S (S m))) ; auto) ;
+      try(rewrite StageSetProperties.ub_le_2 with (m:=1) ; auto ; omega).
+      
+
+      (* depth e > 0 *)
+      rewrite DpthLength1 in H.
+      destruct IHe with (m:=S m) ; auto ; try(omega).
       repeat(split) ; intros ; simpl in *|-*.
-      apply leb_iff in Heqb.
-
+      destruct H1 ; clear H2 IHe.
+      rewrite BKLength ; rewrite BKLength in H0.
+      inversion H1 ; subst ; simpl in *|-*.
+      
       specialize (EqFill1 h v).
       destruct t ; [contradiction|].
-      specialize (EqFill1 ss) ; destruct H3 ; 
       apply EqFill1 ; auto.
-      inversion H3 ; subst ; auto.
-      constructor.
-
-      inversion H4.
-      apply CalculusProperties.depth_svalue in H7 ; exfalso ; omega.
-
-      destruct IHe with (ss:=ss) ; auto ; try(omega).
-      rewrite StageSetProperties.ub_le_2 with (m:=0) ; auto.
-      intros ; left ; apply leb_iff_conv in Heqb ; omega.
-      repeat(split) ; intros ; simpl in *|-*.
-      apply leb_iff_conv in Heqb.
-      rewrite BKLength in H2, H3.
 
       specialize (EqFill2 h v).
       destruct t ; [contradiction|].
-      specialize (EqFill2 ss) ; destruct H3 ; 
       apply EqFill2 ; auto.
-      omega.
-      inversion H3 ; subst ; auto.
-      constructor.
-
-      inversion H4.
-      apply CalculusProperties.depth_svalue in H7 ; exfalso ; omega.
       
-      (* depth e > 1 *)
-      destruct IHe with (ss:=ss) ; auto ; try(omega).
-      rewrite StageSetProperties.ub_le_2 with (m:=(S (length t1))) ; auto.
-      intros ; apply H1 ; omega.
-      repeat(split) ; intros ; simpl in *|-*.
+      destruct H1 ; inversion H1 ; subst ; auto ; constructor.
+      inversion H2 ; subst.
+      apply CalculusProperties.depth_svalue in H5 ; exfalso ; omega.
 
-      specialize (EqFill3 h v).
-      destruct bs ; [exfalso ; simpl in *|-* ; omega|].
-      simpl in *|-*.
-      destruct t ; [contradiction|].
-      rewrite BKLength in H2, H3.
-      
-      specialize (EqFill3 ss) ; destruct H3 ; 
-      apply EqFill3 ; auto.
-      inversion H3 ; subst ; simpl in *|-* ; auto.
-
-      destruct H3 ; inversion H3 ; subst ; simpl in *|-*.
-      rewrite StageSetProperties.ub_remove_equal with 
-        (n:=(S (S (length t1)))) (m:=(S (length t1))) in H14 ; auto.
-      inversion H4.
-      apply CalculusProperties.depth_svalue in H7 ; exfalso ; omega.
-    
     (* EUnbox *)
     destruct bs ; simpl in *|-*.
     specialize (IHe nil h v) ; destruct (trans e).
-    intros ; exfalso ; omega.
+    intros ; destruct m ; exfalso ; omega.
 
     specialize (IHe bs h v).
     specialize (context_stack_not_nil e bs) ; intros CSNotNil.
     specialize (depth_length e bs) ; intros DpthLength.
     specialize (booker_length e bs) ; intros BKLength.
     destruct (trans e) ; intros.
-    rewrite DpthLength in *|-*.
+    destruct m ; [exfalso ; omega| simpl in *|-*].
 
-    unfold eq_ssubst_ss ; repeat(split) ; intros ; simpl in *|-*.
+    unfold eq_ssubst_2 ; repeat(split) ; intros ; simpl in *|-*.
     rewrite MP.ssubst_eunbox, MP.ssubst_evar.
-    simpl in *|-*.
 
-    destruct t ; simpl in *|-*.
- 
-      (* Case depth e = 0 *)
-      destruct H1 ; auto.
-
-      assert(beq_nat (hole_var h) (hole_var n) = false) as BeqFalse1.
-      apply beq_nat_false_iff ; unfold hole_var ; omega.
-      rewrite BeqFalse1 ; simpl ; constructor.
-
-      assert(CRaw.BindingSet.rho 0
-           (StageSet.remove 1 ss) = false) as RhoFalse.
-      rewrite BindingSetProperties.rho_false_mem ; auto.
-      rewrite StageSetProperties.remove_mem_1 ; auto.
-      rewrite RhoFalse ; simpl ; rewrite andb_false_r ; constructor.
-
-      (* Case depth e > 0 *)
-
-      rewrite BKLength in *|-* ; simpl in *|-*.
-
-      remember (ltb h (n + 1)).
-      destruct b ; symmetry in Heqb.
-      assert(CRaw.BindingSet.rho (S (length t0))
-           (StageSet.remove (S (S (length t0))) (StageSet.add (S (length t0)) ss)) = false) as RhoFalse.
-      rewrite BindingSetProperties.rho_false_mem ; auto.
-      rewrite StageSetProperties.remove_mem_1 ; auto.
-      apply StageSetProperties.add_mem_3 ; auto.
-      rewrite RhoFalse ; simpl ; rewrite andb_false_r ; constructor.
-      apply leb_iff_conv in Heqb.
-      assert(beq_nat (hole_var h) (hole_var n) = false) as BeqFalse1.
-      apply beq_nat_false_iff ; unfold hole_var ; omega.
-      rewrite BeqFalse1 ; simpl ; constructor. 
-
-    destruct bs ; simpl in *|-* ; [exfalso ; omega |].
-    simpl in *|-* ; destruct IHe with (ss:=StageSet.remove (S (length t)) ss) ; auto ; try(omega).
-    rewrite <- StageSetProperties.ub_S ; auto.
-    intros ; destruct (length t) ; [exfalso ; omega|] ; simpl.
-    intros ; destruct H1 ; auto.
-    right ; auto.
+    remember (ltb h (n + 1)).
+    destruct b ; symmetry in Heqb ; unfold ltb in Heqb.
+    assert(CRaw.BindingSet.rho m
+           (StageSet.remove (S m) (StageSet.add m ss)) = false) as RhoFalse.
+    rewrite BindingSetProperties.rho_false_mem ; auto.
     rewrite StageSetProperties.remove_mem_1 ; auto.
+    apply StageSetProperties.add_mem_3 ; auto.
+    simpl ; rewrite RhoFalse ; simpl ; rewrite andb_false_r ; constructor.
+    apply leb_iff_conv in Heqb.
+    assert(beq_nat (hole_var h) (hole_var n) = false) as BeqFalse1.
+    apply beq_nat_false_iff ; unfold hole_var ; omega.
+    rewrite BeqFalse1 ; simpl ; constructor. 
 
-    destruct t ; simpl in *|-*.
+    destruct IHe with (m:=m) ; auto ; try(omega).
+    destruct bs ; simpl in *|-*.
+    exfalso ; omega.
+    destruct t ; simpl.
     assert((e0, n) = (e0, (n+length(tl ((e0, n) :: nil)))%nat)) as Eq1.
     rewrite plus_0_r ; auto.
     simpl tl in Eq1.
     rewrite Eq1 ; clear Eq1.
     constructor ; auto.
+    rewrite BKLength in H0 ; simpl in H0.
     repeat(constructor ; auto).
-    unfold eq_ssubst_ss ; intros.
-
-    repeat(constructor ; auto).
+    constructor ; auto.
     assert((e0, n) = (e0, (n+length(tl ((e0, n) :: nil)))%nat)) as Eq1.
     rewrite plus_0_r ; auto.
     simpl tl in Eq1.
     rewrite Eq1 ; clear Eq1.
     constructor ; auto.
-    unfold eq_ssubst_ss ; intros.
-    
-    destruct (length t0) ; auto.
-    rewrite BKLength in H2 ; simpl in H2 ; auto.
+    rewrite BKLength in H0 ; simpl in H0 ; auto.
     constructor.
-
-    destruct H3 ; auto.
-    inversion H2.
+    destruct H1 ; auto.
+    inversion H0.
 
     (* ERun *)
     specialize (IHe bs h v) ;
     destruct (trans e) ; intros ;
-    unfold eq_ssubst_ss ; repeat(split) ; intros ;
-    destruct IHe with (ss:=ss) ; auto.
+    unfold eq_ssubst_2 ; repeat(split) ; intros ;
+    destruct IHe with (m:=m) ; auto.
     rewrite MP.ssubst_bind with (f2:= (fun v0 : T.expr => cast_erun v0)) ; 
     intros.
-    rewrite H2 ; auto.
+    rewrite H1 ; auto.
     rewrite MP.ssubst_erun ; reflexivity.
-    destruct H3 ; auto.
-    inversion H2.
+    destruct H1 ; auto.
+    inversion H0.
 
     (* ELift *)
     specialize (IHe bs h v) ;
     destruct (trans e) ; intros ;
-    unfold eq_ssubst_ss ; repeat(split) ; intros ;
-    destruct IHe with (ss:=ss) ; auto.
+    unfold eq_ssubst_2 ; repeat(split) ; intros ;
+    destruct IHe with (m:=m) ; auto.
     rewrite MP.ssubst_bind with (f2:= (fun v0 : T.expr => cast_elift v0)) ; 
     intros.
-    rewrite H2 ; auto.
+    rewrite H1 ; auto.
     rewrite MP.ssubst_elift ; reflexivity.
-    destruct H3 ; auto.
-    inversion H2.
+    destruct H1 ; auto.
+    inversion H0.
   Qed.
 
   Lemma eq_ssubst_eq:
